<?xml version="1.0" encoding="utf-8"?>
<rdf:RDF
  xmlns:owl="http://www.w3.org/2002/07/owl#"
  xmlns:rdf="http://www.w3.org/1999/02/22-rdf-syntax-ns#"
  xmlns:rdfs="http://www.w3.org/2000/01/rdf-schema#"
>
  <owl:Ontology rdf:about="https://cn.dataone.org/cn/v2/object/ching.11.7">
    <rdfs:label>Embryo Culture and Somatic Embryogenesis from Embryo Culture of Pasania dodonaeifolia Hayata</rdfs:label>
    <rdfs:comment>After cold stratification and husking, the seeds of Pasania dodonaeifolia Hayata, which were collected from Chin Shui Ying and Kuei Tien area, were cultured on MS medium supplemented with growth regulators for three years. The Pasania dodonaeifolia Hayata seeds produced both non-embryogenic callus and embryogenic callus . Embryogenic callus tissue came out for two types: direct embryo and indirect embryo. On the average, it took about50-60 days from the beginning of embryo culture to obvious somatic embryogenesis. Take the âKuei Tien No. 1â seed for example, the germination rate was 19.8%. Root emerged after the seed was cultured for 30 days, shoots came out after 50 days, and normal leaves and twigs grew out after 70 days. Husked Seeds whose diameter was from 4 mm to 12 mm could induce both embryogenic and non-embryogenic callus tissues; the seeds whose diameter was smaller than 3 mm would die after being culture. Seeds were viable only for 3 month after cold stratification. When BA and NAA were used in a 4X6 factorial design experiment, the concentration of NAA significantly influence rooting and embryogenic callus formation, and the most efficacious formulas were 1 mg/L NAA with 0.1 to 1 mg/L BA. Seed diameter and collection area also significantly influence the performance of tissue culture.</rdfs:comment>
  </owl:Ontology>
  <owl:Class rdf:about="https://cn.dataone.org/cn/v2/object/ching.11.7#d_1_a_5">
    <rdfs:label>Table 1. Performance</rdfs:label>
    <rdfs:subClassOf>
      <owl:Restriction rdf:nodeID="Na300d1c084c34421918c4bd153736bcf">
        <owl:onProperty rdf:resource="http://ecoinformatics.org/oboe/oboe.1.1/oboe-core.owl#measuresCharacteristic"/>
        <owl:someValuesFrom rdf:resource="https://cn.dataone.org/cn/v2/object/ching.11.7#d_1_c_5"/>
      </owl:Restriction>
    </rdfs:subClassOf>
    <rdfs:subClassOf rdf:resource="http://ecoinformatics.org/oboe/oboe.1.1/oboe-core.owl#MeasurementType"/>
    <rdfs:subClassOf>
      <owl:Restriction rdf:nodeID="N50722aa36b2d4082b19bf21c4c5aaecd">
        <owl:onProperty rdf:resource="http://ecoinformatics.org/oboe/oboe.1.1/oboe-core.owl#measuresEntity"/>
        <owl:someValuesFrom rdf:resource="https://cn.dataone.org/cn/v2/object/ching.11.7#d_1"/>
      </owl:Restriction>
    </rdfs:subClassOf>
  </owl:Class>
  <owl:Class rdf:about="https://cn.dataone.org/cn/v2/object/ching.11.7#d_1_a_3">
    <rdfs:subClassOf>
      <owl:Restriction rdf:nodeID="N2b0bc1acb0e4413d8324fe852f021371">
        <owl:onProperty rdf:resource="http://ecoinformatics.org/oboe/oboe.1.1/oboe-core.owl#measuresEntity"/>
        <owl:someValuesFrom rdf:resource="https://cn.dataone.org/cn/v2/object/ching.11.7#d_1"/>
      </owl:Restriction>
    </rdfs:subClassOf>
    <rdfs:subClassOf rdf:resource="http://ecoinformatics.org/oboe/oboe.1.1/oboe-core.owl#MeasurementType"/>
    <rdfs:label>Table 1. Performance</rdfs:label>
    <rdfs:subClassOf>
      <owl:Restriction rdf:nodeID="N9abc4dcc2f704c65aa2f18cb959f6cbf">
        <owl:someValuesFrom rdf:resource="https://cn.dataone.org/cn/v2/object/ching.11.7#d_1_c_3"/>
        <owl:onProperty rdf:resource="http://ecoinformatics.org/oboe/oboe.1.1/oboe-core.owl#measuresCharacteristic"/>
      </owl:Restriction>
    </rdfs:subClassOf>
  </owl:Class>
  <owl:Class rdf:about="https://cn.dataone.org/cn/v2/object/ching.11.7#d_1_a_4">
    <rdfs:subClassOf rdf:resource="http://ecoinformatics.org/oboe/oboe.1.1/oboe-core.owl#MeasurementType"/>
    <rdfs:subClassOf>
      <owl:Restriction rdf:nodeID="Nfac642c6aafd42ee896d3bd99100a5ee">
        <owl:onProperty rdf:resource="http://ecoinformatics.org/oboe/oboe.1.1/oboe-core.owl#measuresCharacteristic"/>
        <owl:someValuesFrom rdf:resource="https://cn.dataone.org/cn/v2/object/ching.11.7#d_1_c_4"/>
      </owl:Restriction>
    </rdfs:subClassOf>
    <rdfs:subClassOf>
      <owl:Restriction rdf:nodeID="Ne0554aa702524ed692fba60386f5f31f">
        <owl:someValuesFrom rdf:resource="https://cn.dataone.org/cn/v2/object/ching.11.7#d_1"/>
        <owl:onProperty rdf:resource="http://ecoinformatics.org/oboe/oboe.1.1/oboe-core.owl#measuresEntity"/>
      </owl:Restriction>
    </rdfs:subClassOf>
    <rdfs:label>Table 1. Performance</rdfs:label>
  </owl:Class>
  <owl:Class rdf:about="https://cn.dataone.org/cn/v2/object/ching.11.7#d_1_a_1">
    <rdfs:subClassOf>
      <owl:Restriction rdf:nodeID="Naf201b19ad36449ba884b9f9665a2258">
        <owl:onProperty rdf:resource="http://ecoinformatics.org/oboe/oboe.1.1/oboe-core.owl#measuresCharacteristic"/>
        <owl:someValuesFrom rdf:resource="https://cn.dataone.org/cn/v2/object/ching.11.7#d_1_c_1"/>
      </owl:Restriction>
    </rdfs:subClassOf>
    <rdfs:label>Table 1. Performance</rdfs:label>
    <rdfs:subClassOf>
      <owl:Restriction rdf:nodeID="N6712b17509b742a699f98c0610a7f727">
        <owl:someValuesFrom rdf:resource="https://cn.dataone.org/cn/v2/object/ching.11.7#d_1"/>
        <owl:onProperty rdf:resource="http://ecoinformatics.org/oboe/oboe.1.1/oboe-core.owl#measuresEntity"/>
      </owl:Restriction>
    </rdfs:subClassOf>
    <rdfs:subClassOf rdf:resource="http://ecoinformatics.org/oboe/oboe.1.1/oboe-core.owl#MeasurementType"/>
  </owl:Class>
  <owl:Class rdf:about="https://cn.dataone.org/cn/v2/object/ching.11.7#d_1_a_2">
    <rdfs:label>Table 1. Performance</rdfs:label>
    <rdfs:subClassOf>
      <owl:Restriction rdf:nodeID="Ne77f7553e83945fa88d3b04499d56755">
        <owl:onProperty rdf:resource="http://ecoinformatics.org/oboe/oboe.1.1/oboe-core.owl#measuresCharacteristic"/>
        <owl:someValuesFrom rdf:resource="https://cn.dataone.org/cn/v2/object/ching.11.7#d_1_c_2"/>
      </owl:Restriction>
    </rdfs:subClassOf>
    <rdfs:subClassOf rdf:resource="http://ecoinformatics.org/oboe/oboe.1.1/oboe-core.owl#MeasurementType"/>
    <rdfs:subClassOf>
      <owl:Restriction rdf:nodeID="Nf363de62f3ce42c5b9d21584d5879d31">
        <owl:onProperty rdf:resource="http://ecoinformatics.org/oboe/oboe.1.1/oboe-core.owl#measuresEntity"/>
        <owl:someValuesFrom rdf:resource="https://cn.dataone.org/cn/v2/object/ching.11.7#d_1"/>
      </owl:Restriction>
    </rdfs:subClassOf>
  </owl:Class>
  <owl:Class rdf:about="https://cn.dataone.org/cn/v2/object/ching.11.7#d_1_c_4">
    <rdfs:label>Performance</rdfs:label>
    <rdfs:subClassOf rdf:resource="http://ecoinformatics.org/oboe/oboe.1.1/oboe-core.owl#Characteristic"/>
    <rdfs:comment>the performance of tissue culture of Pasania dodonaeifolia Hayata seed.</rdfs:comment>
  </owl:Class>
  <owl:Class rdf:about="https://cn.dataone.org/cn/v2/object/ching.11.7#d_1_c_2">
    <rdfs:label>Performance</rdfs:label>
    <rdfs:comment>the performance of tissue culture of Pasania dodonaeifolia Hayata seed.</rdfs:comment>
    <rdfs:subClassOf rdf:resource="http://ecoinformatics.org/oboe/oboe.1.1/oboe-core.owl#Characteristic"/>
  </owl:Class>
  <owl:Class rdf:about="https://cn.dataone.org/cn/v2/object/ching.11.7#d_1_c_5">
    <rdfs:label>Performance</rdfs:label>
    <rdfs:subClassOf rdf:resource="http://ecoinformatics.org/oboe/oboe.1.1/oboe-core.owl#Characteristic"/>
    <rdfs:comment>the performance of tissue culture of Pasania dodonaeifolia Hayata seed.</rdfs:comment>
  </owl:Class>
  <owl:Class rdf:about="https://cn.dataone.org/cn/v2/object/ching.11.7#d_1_c_3">
    <rdfs:subClassOf rdf:resource="http://ecoinformatics.org/oboe/oboe.1.1/oboe-core.owl#Characteristic"/>
    <rdfs:label>Performance</rdfs:label>
    <rdfs:comment>the performance of tissue culture of Pasania dodonaeifolia Hayata seed.</rdfs:comment>
  </owl:Class>
  <owl:Class rdf:about="https://cn.dataone.org/cn/v2/object/ching.11.7#d_1">
    <rdfs:subClassOf rdf:resource="http://ecoinformatics.org/oboe/oboe.1.1/oboe-core.owl#Entity"/>
    <rdfs:label>Table 1.</rdfs:label>
    <rdfs:comment>Effect of seed diameter on the performance of tissue culture of Pasania dodonaeifolia Hayata seed.(Values within the same line with same letter are no significantly difference according to 5ï¹ªDuncanâs multiple range testã)</rdfs:comment>
  </owl:Class>
  <owl:Class rdf:about="https://cn.dataone.org/cn/v2/object/ching.11.7#d_1_c_1">
    <rdfs:comment>the performance of tissue culture of Pasania dodonaeifolia Hayata seed.</rdfs:comment>
    <rdfs:subClassOf rdf:resource="http://ecoinformatics.org/oboe/oboe.1.1/oboe-core.owl#Characteristic"/>
    <rdfs:label>Performance</rdfs:label>
  </owl:Class>
</rdf:RDF>
