<?xml version="1.0" encoding="utf-8"?>
<rdf:RDF
  xmlns:owl="http://www.w3.org/2002/07/owl#"
  xmlns:rdf="http://www.w3.org/1999/02/22-rdf-syntax-ns#"
  xmlns:rdfs="http://www.w3.org/2000/01/rdf-schema#"
>
  <owl:Class rdf:about="https://cn.dataone.org/cn/v2/object/doi:10.5063/F1TD9V7X#d_1_a_2">
    <rdfs:label>freshwaterDischargeSewardAK_1930_2008.csv </rdfs:label>
    <rdfs:subClassOf>
      <owl:Restriction rdf:nodeID="Ne013f96299cb45fd91a4d962cf942f81">
        <owl:onProperty rdf:resource="http://ecoinformatics.org/oboe/oboe.1.1/oboe-core.owl#measuresEntity"/>
        <owl:someValuesFrom rdf:resource="https://cn.dataone.org/cn/v2/object/doi:10.5063/F1TD9V7X#d_1"/>
      </owl:Restriction>
    </rdfs:subClassOf>
    <rdfs:subClassOf>
      <owl:Restriction rdf:nodeID="N0c96e9c3c34b4550bb73b45c1fdcf6aa">
        <owl:someValuesFrom rdf:resource="https://cn.dataone.org/cn/v2/object/doi:10.5063/F1TD9V7X#d_1_c_2"/>
        <owl:onProperty rdf:resource="http://ecoinformatics.org/oboe/oboe.1.1/oboe-core.owl#measuresCharacteristic"/>
      </owl:Restriction>
    </rdfs:subClassOf>
    <rdfs:subClassOf rdf:resource="http://ecoinformatics.org/oboe/oboe.1.1/oboe-core.owl#MeasurementType"/>
  </owl:Class>
  <owl:Class rdf:about="https://cn.dataone.org/cn/v2/object/doi:10.5063/F1TD9V7X#d_1_a_6">
    <rdfs:label>freshwaterDischargeSewardAK_1930_2008.csv </rdfs:label>
    <rdfs:subClassOf>
      <owl:Restriction rdf:nodeID="N9592bf19880f4288a373f29dc728949e">
        <owl:someValuesFrom rdf:resource="https://cn.dataone.org/cn/v2/object/doi:10.5063/F1TD9V7X#d_1_c_6"/>
        <owl:onProperty rdf:resource="http://ecoinformatics.org/oboe/oboe.1.1/oboe-core.owl#measuresCharacteristic"/>
      </owl:Restriction>
    </rdfs:subClassOf>
    <rdfs:subClassOf rdf:resource="http://ecoinformatics.org/oboe/oboe.1.1/oboe-core.owl#MeasurementType"/>
    <rdfs:subClassOf>
      <owl:Restriction rdf:nodeID="N12fb12f0e3374d0180081800debab6e8">
        <owl:someValuesFrom rdf:resource="https://cn.dataone.org/cn/v2/object/doi:10.5063/F1TD9V7X#d_1"/>
        <owl:onProperty rdf:resource="http://ecoinformatics.org/oboe/oboe.1.1/oboe-core.owl#measuresEntity"/>
      </owl:Restriction>
    </rdfs:subClassOf>
  </owl:Class>
  <owl:Class rdf:about="https://cn.dataone.org/cn/v2/object/doi:10.5063/F1TD9V7X#d_1_a_3">
    <rdfs:subClassOf>
      <owl:Restriction rdf:nodeID="N7ec0973b87a04e28bda15048e1772268">
        <owl:onProperty rdf:resource="http://ecoinformatics.org/oboe/oboe.1.1/oboe-core.owl#measuresEntity"/>
        <owl:someValuesFrom rdf:resource="https://cn.dataone.org/cn/v2/object/doi:10.5063/F1TD9V7X#d_1"/>
      </owl:Restriction>
    </rdfs:subClassOf>
    <rdfs:subClassOf rdf:resource="http://ecoinformatics.org/oboe/oboe.1.1/oboe-core.owl#MeasurementType"/>
    <rdfs:label>freshwaterDischargeSewardAK_1930_2008.csv </rdfs:label>
    <rdfs:subClassOf>
      <owl:Restriction rdf:nodeID="N897d2ae3465b45cc84025991ca61493a">
        <owl:someValuesFrom rdf:resource="https://cn.dataone.org/cn/v2/object/doi:10.5063/F1TD9V7X#d_1_c_3"/>
        <owl:onProperty rdf:resource="http://ecoinformatics.org/oboe/oboe.1.1/oboe-core.owl#measuresCharacteristic"/>
      </owl:Restriction>
    </rdfs:subClassOf>
  </owl:Class>
  <owl:Class rdf:about="https://cn.dataone.org/cn/v2/object/doi:10.5063/F1TD9V7X#d_1_a_4">
    <rdfs:subClassOf rdf:resource="http://ecoinformatics.org/oboe/oboe.1.1/oboe-core.owl#MeasurementType"/>
    <rdfs:label>freshwaterDischargeSewardAK_1930_2008.csv </rdfs:label>
    <rdfs:subClassOf>
      <owl:Restriction rdf:nodeID="Nb5650a2260414eb1a1ff258a15d20b2c">
        <owl:onProperty rdf:resource="http://ecoinformatics.org/oboe/oboe.1.1/oboe-core.owl#measuresCharacteristic"/>
        <owl:someValuesFrom rdf:resource="https://cn.dataone.org/cn/v2/object/doi:10.5063/F1TD9V7X#d_1_c_4"/>
      </owl:Restriction>
    </rdfs:subClassOf>
    <rdfs:subClassOf>
      <owl:Restriction rdf:nodeID="N2962b2da97e94a0e8d798eee970af647">
        <owl:onProperty rdf:resource="http://ecoinformatics.org/oboe/oboe.1.1/oboe-core.owl#measuresEntity"/>
        <owl:someValuesFrom rdf:resource="https://cn.dataone.org/cn/v2/object/doi:10.5063/F1TD9V7X#d_1"/>
      </owl:Restriction>
    </rdfs:subClassOf>
  </owl:Class>
  <owl:Class rdf:about="https://cn.dataone.org/cn/v2/object/doi:10.5063/F1TD9V7X#d_1_a_7">
    <rdfs:subClassOf>
      <owl:Restriction rdf:nodeID="Nfc969c80cdde4d53800910af285434c5">
        <owl:someValuesFrom rdf:resource="https://cn.dataone.org/cn/v2/object/doi:10.5063/F1TD9V7X#d_1"/>
        <owl:onProperty rdf:resource="http://ecoinformatics.org/oboe/oboe.1.1/oboe-core.owl#measuresEntity"/>
      </owl:Restriction>
    </rdfs:subClassOf>
    <rdfs:subClassOf rdf:resource="http://ecoinformatics.org/oboe/oboe.1.1/oboe-core.owl#MeasurementType"/>
    <rdfs:label>freshwaterDischargeSewardAK_1930_2008.csv </rdfs:label>
    <rdfs:subClassOf>
      <owl:Restriction rdf:nodeID="N8c1cd212f90f4fb8b154ffee98b3ff45">
        <owl:onProperty rdf:resource="http://ecoinformatics.org/oboe/oboe.1.1/oboe-core.owl#measuresCharacteristic"/>
        <owl:someValuesFrom rdf:resource="https://cn.dataone.org/cn/v2/object/doi:10.5063/F1TD9V7X#d_1_c_7"/>
      </owl:Restriction>
    </rdfs:subClassOf>
  </owl:Class>
  <owl:Class rdf:about="https://cn.dataone.org/cn/v2/object/doi:10.5063/F1TD9V7X#d_1_a_1">
    <rdfs:subClassOf rdf:resource="http://ecoinformatics.org/oboe/oboe.1.1/oboe-core.owl#MeasurementType"/>
    <rdfs:subClassOf>
      <owl:Restriction rdf:nodeID="N06a5a126afd942ec8408f7d99ec7676c">
        <owl:someValuesFrom rdf:resource="https://cn.dataone.org/cn/v2/object/doi:10.5063/F1TD9V7X#d_1"/>
        <owl:onProperty rdf:resource="http://ecoinformatics.org/oboe/oboe.1.1/oboe-core.owl#measuresEntity"/>
      </owl:Restriction>
    </rdfs:subClassOf>
    <rdfs:label>freshwaterDischargeSewardAK_1930_2008.csv </rdfs:label>
    <rdfs:subClassOf>
      <owl:Restriction rdf:nodeID="Nbbff8ccd7f2241c685ffdf7510534f39">
        <owl:someValuesFrom rdf:resource="https://cn.dataone.org/cn/v2/object/doi:10.5063/F1TD9V7X#d_1_c_1"/>
        <owl:onProperty rdf:resource="http://ecoinformatics.org/oboe/oboe.1.1/oboe-core.owl#measuresCharacteristic"/>
      </owl:Restriction>
    </rdfs:subClassOf>
  </owl:Class>
  <owl:Ontology rdf:about="https://cn.dataone.org/cn/v2/object/doi:10.5063/F1TD9V7X">
    <rdfs:comment>This program continues a 40(+) year time series of temperature and salinity measurements at hydrographic station GAK 1. The data set, which began in 1970, now consists of monthly CTDs and a mooring with 6 - 7 temperature/conductivity recorders throughout the water column, a fluorometer and nitrate sensor at 20 m depth and a nitrate sensor at 150 m depth. The project monitors five important Alaska Coastal Current ecosystem parameters and to quantify and understand interannual and longer period variability in: 

1. Temperature and salinity throughout the 250 m deep water column, 2. Near surface stratification, 3. Near and subsurface nitrate supply on the inner shelf, 4. Fluorescence as an index of phytoplankton biomass, and 5. Atmosphere-ocean heat fluxes. 

In aggregate these variables are basic descriptors of the Alaska Coastal Current, an important habitat and migratory corridor for organisms inhabiting the northern Gulf of Alaska, including Prince William Sound. 

Data here spans 1970 - 2012. ON GOING DATA CAN BE ACCESSED AT THE UAF GAK1 WEBSITE: http://www.ims.uaf.edu/gak1/

*****Publications which have cited this data: 

--Janout, M. A., T. J. Weingartner, T. C. Royer, and S. L. Danielson, 2010, On the nature of winter cooling and the recent temperature shift on the northern Gulf of Alaska shelf, J. Geophys. Res., 115, C05023, doi:10.1029/2009JC005774. 

--Bechtol, W.R., 2009. Abundance, recruitment, and environmental forcing of Kodiak red king crab. University of Alaska Fairbanks, Doctoral dissertation, 205 p 

--Tribuzio, C.A.,. 2009. Life history, demography and ecology of the spiny dogfish (Squalus acanthias) in the Gulf of Alaska: Critical information for aiding management. University of Alaska Fairbanks, Doctoral dissertation, in prep. 

--Ebbesmeyer, C. C., W. J. Ingraham, T. C. Royer, and C. E. Grosch, 2007, Tub Toys Orbit the Pacific Subarctic Gyre, Eos Trans. AGU, 88(1), 1. 

--Sarkar, N., 2007, Mixed layer dynamics along the Seward Line in the northern Gulf of Alaska, Ph.D. dissertation, Old Dominion University, Norfolk, VA, 71p. 

--Schroeder, I. D., 2007, Annual and interannual variability in the wind field and hydrography along the Seward Line in the northern Gulf of Alaska, Ph.D. dissertation, Old Dominion University, Norfolk, VA, 81p. 

--Royer, T. C. and C. E. Grosch, 2006, Ocean warming and freshening in the northern Gulf of Alaska, Geophysical Research Letters, 33 (16), L16605,doi:10.1029/2006GL026767 

--Capotondi, A., M. A. Alexander, C. Deser and A. J. Miller, 2005, Low-Frequency Pycnocline Variability in the Northeast Pacific, Journal of Physical Oceanography, V. 35, 8, 1403-1420 

--Ingolfsson, A., 2005, Community structure and zonation patterns of rocky shores at high latitudes: an interocean comparison, Journal of Biogeography, 32(1), 169-182, doi:10.1111/j.1365-2699.2004.01150.x 

--Royer, T.C., 2005, Hydrographic responses at a coastal site in the northern Gulf of Alaska to seasonal and interannual forcing, Deep-Sea Research Part II-Topical Studies in Oceanography, 52 (1-2): 267-288 

--Sarkar, N, T. C. Royer and C. E. Grosch, 2005. Hydrographic and mixed layer depth variability on the shelf in the northern Gulf of Alaska, 1974-1998. Cont. Shelf. Res. 25: 2147 - 2162. 

--Weingartner, T.J., Danielson, S.L. and Royer, T.C., 2005, Freshwater variability and predictability in the Alaska Coastal Current, Deep-Sea Research Part II-Topical Studies in Oceanography, 52 (1-2): 169-191

--Mueter, F.J., 2004, Gulf of Alaska - Marine Ecosystems of the North Pacific, Vol. PICES Special Publication 1 (pp. 153-175): PICES Special Publication 1.

--Stabeno, P.J., N.A. Bond, A.J. Hermann, N.B. Kachel, C.W. Mordy and J.E. Overland, 2004, Meteorology and oceanography of the Northern Gulf of Alaska, Continental Shelf Research, 24, 859-879

--PICES, 2004. Marine Ecosystems of the North Pacific. PICES Special Publication 1, 280p.

--Committee to Review the Gulf of Alaska Ecosystem Monitoring Program, National Research Council, 2002, A Century of Ecosystem Science - Planning Long-Term Research in the Gulf of Alaska, National Research Council, National Academy Press, Washington, D.C.

--Boldt, J. L. and L. J. Haldorson, 2002 A Bioenergetics Approach to Estimating Consumption of Zooplankton by Juvenile Pink Salmn in Prince William Sound, Alaska, Alaska Fishery Research Bulletin, V9 No. 2, Winter 2002

--Royer, T.C., Grosch, C.E., and Mysak, L.A., 2001, Interdecadal variability of Northeast Pacific coastal freshwater and its implications on biological productivity, Progress in Oceanography, 49 (1-4): 95-111 Sp. Iss. SI

--Mueter, F.J., 1999, Spatial and temporal patterns in the Gulf of Alaska groundfish community in relation to the environments, Doctoral dissertation

--Parker, K.S., T.C. Royer, and R.B. Deriso, 1995. High latitude climate forcing by the 18.6 year lunar nodal cycle and historical recruitment trends in Pacific halibut, Can. Spec. Publ. Fish. Aquat. Sci., 121:447-459.

--Muter, F.J., B.L. Norcross and T.C. Royer, 1994. Do cyclic temperatures cause cyclic fisheries?, Can. Spec. Publ. Fish. Aquat. Sci., 121:119-129.

--Royer, T.C. 1993. High-latitude oceanic variability associated with the 18.6-year nodal tide. J. Geop. Res., 98:4639-4644.

--Royer, T.C. 1989. Upper ocean temperature variability in the Northeast Pacific Ocean: Is it an indicator of global warming? J. Geop. Res., 94:18175-18183.

--Xiong, Q. and T.C. Royer. 1984. Coastal temperature and salinity in the northern Gulf of Alaska, J. Geop. Res., 89:8061-8066.</rdfs:comment>
    <rdfs:label>Toward Long-Term Monitoring of the Gulf of Alaska Ecosystem, GAK1 Mooring Freshwater Discharge data, Seward, Alaska (1970-2012)</rdfs:label>
  </owl:Ontology>
  <owl:Class rdf:about="https://cn.dataone.org/cn/v2/object/doi:10.5063/F1TD9V7X#d_1_a_5">
    <rdfs:subClassOf rdf:resource="http://ecoinformatics.org/oboe/oboe.1.1/oboe-core.owl#MeasurementType"/>
    <rdfs:label>freshwaterDischargeSewardAK_1930_2008.csv </rdfs:label>
    <rdfs:subClassOf>
      <owl:Restriction rdf:nodeID="Ndf54fc9c27b44dea8eb15859b8cb5862">
        <owl:onProperty rdf:resource="http://ecoinformatics.org/oboe/oboe.1.1/oboe-core.owl#measuresEntity"/>
        <owl:someValuesFrom rdf:resource="https://cn.dataone.org/cn/v2/object/doi:10.5063/F1TD9V7X#d_1"/>
      </owl:Restriction>
    </rdfs:subClassOf>
    <rdfs:subClassOf>
      <owl:Restriction rdf:nodeID="Nada009172b8d4ccd828aa648edbe2a02">
        <owl:onProperty rdf:resource="http://ecoinformatics.org/oboe/oboe.1.1/oboe-core.owl#measuresCharacteristic"/>
        <owl:someValuesFrom rdf:resource="https://cn.dataone.org/cn/v2/object/doi:10.5063/F1TD9V7X#d_1_c_5"/>
      </owl:Restriction>
    </rdfs:subClassOf>
  </owl:Class>
  <owl:Class rdf:about="https://cn.dataone.org/cn/v2/object/doi:10.5063/F1TD9V7X#d_1_c_1">
    <rdfs:subClassOf rdf:resource="http://ecoinformatics.org/oboe/oboe.1.1/oboe-core.owl#Characteristic"/>
    <rdfs:comment>Decimal year (year.fraction of year) Fractions begin Jan 1 of given year.</rdfs:comment>
  </owl:Class>
  <owl:Class rdf:about="https://cn.dataone.org/cn/v2/object/doi:10.5063/F1TD9V7X#d_1_c_7">
    <rdfs:subClassOf rdf:resource="http://ecoinformatics.org/oboe/oboe.1.1/oboe-core.owl#Characteristic"/>
    <rdfs:comment>Decimal year (year.fraction of year) Fractions begin Jan 1 of given year.</rdfs:comment>
  </owl:Class>
  <owl:Class rdf:about="https://cn.dataone.org/cn/v2/object/doi:10.5063/F1TD9V7X#d_1_c_6">
    <rdfs:subClassOf rdf:resource="http://ecoinformatics.org/oboe/oboe.1.1/oboe-core.owl#Characteristic"/>
    <rdfs:comment>Decimal year (year.fraction of year) Fractions begin Jan 1 of given year.</rdfs:comment>
  </owl:Class>
  <owl:Class rdf:about="https://cn.dataone.org/cn/v2/object/doi:10.5063/F1TD9V7X#d_1">
    <rdfs:subClassOf rdf:resource="http://ecoinformatics.org/oboe/oboe.1.1/oboe-core.owl#Entity"/>
    <rdfs:label>freshwaterDischargeSewardAK_1930_2008.csv</rdfs:label>
  </owl:Class>
  <owl:Class rdf:about="https://cn.dataone.org/cn/v2/object/doi:10.5063/F1TD9V7X#d_1_c_5">
    <rdfs:comment>Decimal year (year.fraction of year) Fractions begin Jan 1 of given year.</rdfs:comment>
    <rdfs:subClassOf rdf:resource="http://ecoinformatics.org/oboe/oboe.1.1/oboe-core.owl#Characteristic"/>
  </owl:Class>
  <owl:Class rdf:about="https://cn.dataone.org/cn/v2/object/doi:10.5063/F1TD9V7X#d_1_c_2">
    <rdfs:comment>Decimal year (year.fraction of year) Fractions begin Jan 1 of given year.</rdfs:comment>
    <rdfs:subClassOf rdf:resource="http://ecoinformatics.org/oboe/oboe.1.1/oboe-core.owl#Characteristic"/>
  </owl:Class>
  <owl:Class rdf:about="https://cn.dataone.org/cn/v2/object/doi:10.5063/F1TD9V7X#d_1_c_4">
    <rdfs:comment>Decimal year (year.fraction of year) Fractions begin Jan 1 of given year.</rdfs:comment>
    <rdfs:subClassOf rdf:resource="http://ecoinformatics.org/oboe/oboe.1.1/oboe-core.owl#Characteristic"/>
  </owl:Class>
  <owl:Class rdf:about="https://cn.dataone.org/cn/v2/object/doi:10.5063/F1TD9V7X#d_1_c_3">
    <rdfs:subClassOf rdf:resource="http://ecoinformatics.org/oboe/oboe.1.1/oboe-core.owl#Characteristic"/>
    <rdfs:comment>Decimal year (year.fraction of year) Fractions begin Jan 1 of given year.</rdfs:comment>
  </owl:Class>
</rdf:RDF>
