<?xml version="1.0" encoding="utf-8"?>
<rdf:RDF
  xmlns:owl="http://www.w3.org/2002/07/owl#"
  xmlns:rdf="http://www.w3.org/1999/02/22-rdf-syntax-ns#"
  xmlns:rdfs="http://www.w3.org/2000/01/rdf-schema#"
>
  <owl:Class rdf:about="https://cn.dataone.org/cn/v2/object/doi:10.5063/AA/nceas.196.3#d_1_a_8">
    <rdfs:label>Macroecological database of mammalian body mass Continent</rdfs:label>
    <rdfs:subClassOf rdf:resource="http://ecoinformatics.org/oboe/oboe.1.1/oboe-core.owl#MeasurementType"/>
    <rdfs:subClassOf>
      <owl:Restriction rdf:nodeID="Nccc1a4fa45c642db803839d77a1d5af0">
        <owl:someValuesFrom rdf:resource="https://cn.dataone.org/cn/v2/object/doi:10.5063/AA/nceas.196.3#d_1"/>
        <owl:onProperty rdf:resource="http://ecoinformatics.org/oboe/oboe.1.1/oboe-core.owl#measuresEntity"/>
      </owl:Restriction>
    </rdfs:subClassOf>
    <rdfs:subClassOf>
      <owl:Restriction rdf:nodeID="N5410c77ceddc4871ad7640a2f06eb912">
        <owl:someValuesFrom rdf:resource="https://cn.dataone.org/cn/v2/object/doi:10.5063/AA/nceas.196.3#d_1_c_8"/>
        <owl:onProperty rdf:resource="http://ecoinformatics.org/oboe/oboe.1.1/oboe-core.owl#measuresCharacteristic"/>
      </owl:Restriction>
    </rdfs:subClassOf>
  </owl:Class>
  <owl:Class rdf:about="https://cn.dataone.org/cn/v2/object/doi:10.5063/AA/nceas.196.3#d_1_a_4">
    <rdfs:subClassOf rdf:resource="http://ecoinformatics.org/oboe/oboe.1.1/oboe-core.owl#MeasurementType"/>
    <rdfs:subClassOf>
      <owl:Restriction rdf:nodeID="Nd527a80c9cff45bdbbdc0489749e3ead">
        <owl:onProperty rdf:resource="http://ecoinformatics.org/oboe/oboe.1.1/oboe-core.owl#measuresEntity"/>
        <owl:someValuesFrom rdf:resource="https://cn.dataone.org/cn/v2/object/doi:10.5063/AA/nceas.196.3#d_1"/>
      </owl:Restriction>
    </rdfs:subClassOf>
    <rdfs:label>Macroecological database of mammalian body mass Continent</rdfs:label>
    <rdfs:subClassOf>
      <owl:Restriction rdf:nodeID="N093467ed93244677b29ad1ef7ad3b285">
        <owl:onProperty rdf:resource="http://ecoinformatics.org/oboe/oboe.1.1/oboe-core.owl#measuresCharacteristic"/>
        <owl:someValuesFrom rdf:resource="https://cn.dataone.org/cn/v2/object/doi:10.5063/AA/nceas.196.3#d_1_c_4"/>
      </owl:Restriction>
    </rdfs:subClassOf>
  </owl:Class>
  <owl:Class rdf:about="https://cn.dataone.org/cn/v2/object/doi:10.5063/AA/nceas.196.3#d_1_a_3">
    <rdfs:subClassOf rdf:resource="http://ecoinformatics.org/oboe/oboe.1.1/oboe-core.owl#MeasurementType"/>
    <rdfs:subClassOf>
      <owl:Restriction rdf:nodeID="Ndcbc99954bc64a23970e3d840a68e242">
        <owl:someValuesFrom rdf:resource="https://cn.dataone.org/cn/v2/object/doi:10.5063/AA/nceas.196.3#d_1_c_3"/>
        <owl:onProperty rdf:resource="http://ecoinformatics.org/oboe/oboe.1.1/oboe-core.owl#measuresCharacteristic"/>
      </owl:Restriction>
    </rdfs:subClassOf>
    <rdfs:label>Macroecological database of mammalian body mass Continent</rdfs:label>
    <rdfs:subClassOf>
      <owl:Restriction rdf:nodeID="N3d3997451f9e4a69be512989912298cb">
        <owl:someValuesFrom rdf:resource="https://cn.dataone.org/cn/v2/object/doi:10.5063/AA/nceas.196.3#d_1"/>
        <owl:onProperty rdf:resource="http://ecoinformatics.org/oboe/oboe.1.1/oboe-core.owl#measuresEntity"/>
      </owl:Restriction>
    </rdfs:subClassOf>
  </owl:Class>
  <owl:Class rdf:about="https://cn.dataone.org/cn/v2/object/doi:10.5063/AA/nceas.196.3#d_1_a_2">
    <rdfs:subClassOf>
      <owl:Restriction rdf:nodeID="N0d9a25bb1250423b8ddd794e7c44a002">
        <owl:someValuesFrom rdf:resource="https://cn.dataone.org/cn/v2/object/doi:10.5063/AA/nceas.196.3#d_1"/>
        <owl:onProperty rdf:resource="http://ecoinformatics.org/oboe/oboe.1.1/oboe-core.owl#measuresEntity"/>
      </owl:Restriction>
    </rdfs:subClassOf>
    <rdfs:label>Macroecological database of mammalian body mass Continent</rdfs:label>
    <rdfs:subClassOf rdf:resource="http://ecoinformatics.org/oboe/oboe.1.1/oboe-core.owl#MeasurementType"/>
    <rdfs:subClassOf>
      <owl:Restriction rdf:nodeID="N341a1d87fd31490b851c65bf70404a82">
        <owl:someValuesFrom rdf:resource="https://cn.dataone.org/cn/v2/object/doi:10.5063/AA/nceas.196.3#d_1_c_2"/>
        <owl:onProperty rdf:resource="http://ecoinformatics.org/oboe/oboe.1.1/oboe-core.owl#measuresCharacteristic"/>
      </owl:Restriction>
    </rdfs:subClassOf>
  </owl:Class>
  <owl:Class rdf:about="https://cn.dataone.org/cn/v2/object/doi:10.5063/AA/nceas.196.3#d_1_a_7">
    <rdfs:subClassOf>
      <owl:Restriction rdf:nodeID="N0fceb4bc3b864b70a6c247cdbe394391">
        <owl:someValuesFrom rdf:resource="https://cn.dataone.org/cn/v2/object/doi:10.5063/AA/nceas.196.3#d_1"/>
        <owl:onProperty rdf:resource="http://ecoinformatics.org/oboe/oboe.1.1/oboe-core.owl#measuresEntity"/>
      </owl:Restriction>
    </rdfs:subClassOf>
    <rdfs:label>Macroecological database of mammalian body mass Continent</rdfs:label>
    <rdfs:subClassOf rdf:resource="http://ecoinformatics.org/oboe/oboe.1.1/oboe-core.owl#MeasurementType"/>
    <rdfs:subClassOf>
      <owl:Restriction rdf:nodeID="N89852e66e88f46c1aa0f0fe81488fde9">
        <owl:someValuesFrom rdf:resource="https://cn.dataone.org/cn/v2/object/doi:10.5063/AA/nceas.196.3#d_1_c_7"/>
        <owl:onProperty rdf:resource="http://ecoinformatics.org/oboe/oboe.1.1/oboe-core.owl#measuresCharacteristic"/>
      </owl:Restriction>
    </rdfs:subClassOf>
  </owl:Class>
  <owl:Class rdf:about="https://cn.dataone.org/cn/v2/object/doi:10.5063/AA/nceas.196.3#d_1_a_1">
    <rdfs:subClassOf>
      <owl:Restriction rdf:nodeID="Nd19db589ff214b2495f75afc87c11983">
        <owl:onProperty rdf:resource="http://ecoinformatics.org/oboe/oboe.1.1/oboe-core.owl#measuresEntity"/>
        <owl:someValuesFrom rdf:resource="https://cn.dataone.org/cn/v2/object/doi:10.5063/AA/nceas.196.3#d_1"/>
      </owl:Restriction>
    </rdfs:subClassOf>
    <rdfs:label>Macroecological database of mammalian body mass Continent</rdfs:label>
    <rdfs:subClassOf rdf:resource="http://ecoinformatics.org/oboe/oboe.1.1/oboe-core.owl#MeasurementType"/>
    <rdfs:subClassOf>
      <owl:Restriction rdf:nodeID="Nf195c633babb43d39aa43e9b13c6ab78">
        <owl:onProperty rdf:resource="http://ecoinformatics.org/oboe/oboe.1.1/oboe-core.owl#measuresCharacteristic"/>
        <owl:someValuesFrom rdf:resource="https://cn.dataone.org/cn/v2/object/doi:10.5063/AA/nceas.196.3#d_1_c_1"/>
      </owl:Restriction>
    </rdfs:subClassOf>
  </owl:Class>
  <owl:Class rdf:about="https://cn.dataone.org/cn/v2/object/doi:10.5063/AA/nceas.196.3#d_2_a_1">
    <rdfs:subClassOf>
      <owl:Restriction rdf:nodeID="N71a57fc2ba994ae48a386387a42ab9bb">
        <owl:onProperty rdf:resource="http://ecoinformatics.org/oboe/oboe.1.1/oboe-core.owl#measuresCharacteristic"/>
        <owl:someValuesFrom rdf:resource="https://cn.dataone.org/cn/v2/object/doi:10.5063/AA/nceas.196.3#d_2_c_1"/>
      </owl:Restriction>
    </rdfs:subClassOf>
    <rdfs:subClassOf rdf:resource="http://ecoinformatics.org/oboe/oboe.1.1/oboe-core.owl#MeasurementType"/>
    <rdfs:label>References Reference number</rdfs:label>
    <rdfs:subClassOf>
      <owl:Restriction rdf:nodeID="N57dc7d6319e04691af030bf75447a543">
        <owl:someValuesFrom rdf:resource="https://cn.dataone.org/cn/v2/object/doi:10.5063/AA/nceas.196.3#d_2"/>
        <owl:onProperty rdf:resource="http://ecoinformatics.org/oboe/oboe.1.1/oboe-core.owl#measuresEntity"/>
      </owl:Restriction>
    </rdfs:subClassOf>
  </owl:Class>
  <owl:Class rdf:about="https://cn.dataone.org/cn/v2/object/doi:10.5063/AA/nceas.196.3#d_1_a_9">
    <rdfs:subClassOf>
      <owl:Restriction rdf:nodeID="Nd0eca5103a474aeeb8c3b8a7c4529b9e">
        <owl:someValuesFrom rdf:resource="https://cn.dataone.org/cn/v2/object/doi:10.5063/AA/nceas.196.3#d_1_c_9"/>
        <owl:onProperty rdf:resource="http://ecoinformatics.org/oboe/oboe.1.1/oboe-core.owl#measuresCharacteristic"/>
      </owl:Restriction>
    </rdfs:subClassOf>
    <rdfs:subClassOf rdf:resource="http://ecoinformatics.org/oboe/oboe.1.1/oboe-core.owl#MeasurementType"/>
    <rdfs:label>Macroecological database of mammalian body mass Continent</rdfs:label>
    <rdfs:subClassOf>
      <owl:Restriction rdf:nodeID="N68349b958b294387826ee9c7f95690b7">
        <owl:someValuesFrom rdf:resource="https://cn.dataone.org/cn/v2/object/doi:10.5063/AA/nceas.196.3#d_1"/>
        <owl:onProperty rdf:resource="http://ecoinformatics.org/oboe/oboe.1.1/oboe-core.owl#measuresEntity"/>
      </owl:Restriction>
    </rdfs:subClassOf>
  </owl:Class>
  <owl:Ontology rdf:about="https://cn.dataone.org/cn/v2/object/doi:10.5063/AA/nceas.196.3">
    <rdfs:comment>The purpose of this data set was to compile body mass information for all mammals on Earth so that we could investigate the patterns of body mass seen across geographic and taxonomic space and evolutionary time.  We were interested in the heritability of body size across taxonomic groups (How conserved is body mass within a genus, family, and order?), in the overall pattern of body mass across continents (Do the moments and other descriptive statistics remain the same across geographic space?), and over evolutionary time (How quickly did body mass patterns iterate on the patterns seen today?  Were the Pleistocene extinctions size specific on each continent, and did these events coincide with the arrival of man?).  These data are also part of a larger project that seeks to integrate body mass patterns across very diverse taxa (NCEAS Working Group on Body size in ecology and paleoecology:  linking pattern and process across space, time and taxonomic scales).  We began with the updated version of Wilson and Reeder's (1993) taxonomic list of all known Recent mammals of the world (N = 4629 species) to which we added status, distribution, and body mass estimates compiled from the primary and secondary literature. Whenever possible, we used an average of male and female body mass, which was in turn averaged over multiple localities to arrive at our species body mass values.  The sources are line referenced in the main data set, with the actual references appearing in a table within the metadata.  Mammals have individual records for each continent they occur on.  Please note that our data set is more than an amalgamation of smaller compilations.  Although we relied heavily a data set for Chiroptera by K. E. Jones (N = 905), the CRC handbook of Mammalian Body Mass (N = 688), and a data set compiled for South America by P. Marquet (N = 505), these total less than half the records in the current database.  The remainder are derived from more than 150 other sources (see reference table).  Furthermore, we include a comprehensive late Pleistocene species assemblage for Africa, North and South America, and Australia (an additional 230 species). "Late Pleistocene" is defined as approximately 11 ka for Africa, North and South America, and as 50 ka for Australia, because these times predate anthropogenic impacts on mammalian fauna. Overall, the temporal coverage is from the late Pleistocene to present (ca. 45,000 ybp to present). Estimates contained within this data set represent a generalized species value, averaged across gender and geographic space.  Consequently, these data are not appropriate for asking population-level questions where the integration of body mass with specific environmental conditions is important.  All extant orders of mammals are included, as well as several archaic groups (N = 4859 species).  Because some species are found on more than one continent (particularly Chiroptera), there are 5731 entries.  We have body masses for the following:  Artiodactyla (280 records), Bibymalagasia (2 records), Carnivora (393 records), Cetacea (75 records), Chiroptera (1071 records), Dasyuromorphia (67 records), Dermoptera (3 records), Didelphimorphia (68 records), Diprotodontia (127 records), Hydracoidea (5 records), Insectivora (234 records), Lagomorpha (53 records), Litopterna (2 records), Macroscelidea (14 records), Microbiotheria (1 record), Monotremata (7 records), Notoryctemorphia (1 record), Notoungulata (5 records), Paucituberculata (5 records), Peramelemorphia (24 records), Perissodactyla (47 records), Pholidota (8 records), Primates (276 records), Proboscidea (14 records), Rodentia (1425 records), Scandentia (15 records), Sirenia (6 records), Tubulidentata (1 record), and Xenarthra (75 records).  

Data has undergone substantial data quality and assurance checking, though this is an on-going process.  Histograms of the body masses of each order were produced, and values at the tails were double-checked for accuracy.  When multiple sources of information were available for a species, or new sources encountered, we used those with higher sample sizes and gender-specific information.

Headers are given here as header name followed by more information such as measurement units or other basic descriptor. More information on the variable definitions can be found in Section B, variable information (at http://www.esapubs.org/archive/ecol/E084/094/metadata.htm). Continent (SA, NA, EA, insular, oceanic, AUS, AF), Status (extinct, historical, introduction, or extant), Order, Family, Genus, Species, Log Mass (grams), Combined Mass (grams), Reference.</rdfs:comment>
    <rdfs:label>Macroecological database of mammalian body mass</rdfs:label>
  </owl:Ontology>
  <owl:Class rdf:about="https://cn.dataone.org/cn/v2/object/doi:10.5063/AA/nceas.196.3#d_1_a_6">
    <rdfs:label>Macroecological database of mammalian body mass Continent</rdfs:label>
    <rdfs:subClassOf>
      <owl:Restriction rdf:nodeID="N5d3a238aa4634634bb2f40119d18d1de">
        <owl:someValuesFrom rdf:resource="https://cn.dataone.org/cn/v2/object/doi:10.5063/AA/nceas.196.3#d_1"/>
        <owl:onProperty rdf:resource="http://ecoinformatics.org/oboe/oboe.1.1/oboe-core.owl#measuresEntity"/>
      </owl:Restriction>
    </rdfs:subClassOf>
    <rdfs:subClassOf rdf:resource="http://ecoinformatics.org/oboe/oboe.1.1/oboe-core.owl#MeasurementType"/>
    <rdfs:subClassOf>
      <owl:Restriction rdf:nodeID="N96a5190be70e4000924f223a5404eec0">
        <owl:someValuesFrom rdf:resource="https://cn.dataone.org/cn/v2/object/doi:10.5063/AA/nceas.196.3#d_1_c_6"/>
        <owl:onProperty rdf:resource="http://ecoinformatics.org/oboe/oboe.1.1/oboe-core.owl#measuresCharacteristic"/>
      </owl:Restriction>
    </rdfs:subClassOf>
  </owl:Class>
  <owl:Class rdf:about="https://cn.dataone.org/cn/v2/object/doi:10.5063/AA/nceas.196.3#d_2_a_2">
    <rdfs:label>References Reference number</rdfs:label>
    <rdfs:subClassOf>
      <owl:Restriction rdf:nodeID="N4f3e6d977cf245b3a25b1b3b66ade5b7">
        <owl:someValuesFrom rdf:resource="https://cn.dataone.org/cn/v2/object/doi:10.5063/AA/nceas.196.3#d_2"/>
        <owl:onProperty rdf:resource="http://ecoinformatics.org/oboe/oboe.1.1/oboe-core.owl#measuresEntity"/>
      </owl:Restriction>
    </rdfs:subClassOf>
    <rdfs:subClassOf rdf:resource="http://ecoinformatics.org/oboe/oboe.1.1/oboe-core.owl#MeasurementType"/>
    <rdfs:subClassOf>
      <owl:Restriction rdf:nodeID="Nd3b5b737317e43fbaf896d1e271f0596">
        <owl:onProperty rdf:resource="http://ecoinformatics.org/oboe/oboe.1.1/oboe-core.owl#measuresCharacteristic"/>
        <owl:someValuesFrom rdf:resource="https://cn.dataone.org/cn/v2/object/doi:10.5063/AA/nceas.196.3#d_2_c_2"/>
      </owl:Restriction>
    </rdfs:subClassOf>
  </owl:Class>
  <owl:Class rdf:about="https://cn.dataone.org/cn/v2/object/doi:10.5063/AA/nceas.196.3#d_3_a_1">
    <rdfs:subClassOf rdf:resource="http://ecoinformatics.org/oboe/oboe.1.1/oboe-core.owl#MeasurementType"/>
    <rdfs:subClassOf>
      <owl:Restriction rdf:nodeID="N99452cf04da141e4a59a3d84013796df">
        <owl:someValuesFrom rdf:resource="https://cn.dataone.org/cn/v2/object/doi:10.5063/AA/nceas.196.3#d_3_c_1"/>
        <owl:onProperty rdf:resource="http://ecoinformatics.org/oboe/oboe.1.1/oboe-core.owl#measuresCharacteristic"/>
      </owl:Restriction>
    </rdfs:subClassOf>
    <rdfs:label>Continental affiliations of mammals Continental affiliations of mammals</rdfs:label>
    <rdfs:subClassOf>
      <owl:Restriction rdf:nodeID="N5732cfd6ecb546108fa8560fb3703aed">
        <owl:someValuesFrom rdf:resource="https://cn.dataone.org/cn/v2/object/doi:10.5063/AA/nceas.196.3#d_3"/>
        <owl:onProperty rdf:resource="http://ecoinformatics.org/oboe/oboe.1.1/oboe-core.owl#measuresEntity"/>
      </owl:Restriction>
    </rdfs:subClassOf>
  </owl:Class>
  <owl:Class rdf:about="https://cn.dataone.org/cn/v2/object/doi:10.5063/AA/nceas.196.3#d_1_a_5">
    <rdfs:subClassOf>
      <owl:Restriction rdf:nodeID="N76fdd25f55694f87b96f22b3697df3ab">
        <owl:onProperty rdf:resource="http://ecoinformatics.org/oboe/oboe.1.1/oboe-core.owl#measuresCharacteristic"/>
        <owl:someValuesFrom rdf:resource="https://cn.dataone.org/cn/v2/object/doi:10.5063/AA/nceas.196.3#d_1_c_5"/>
      </owl:Restriction>
    </rdfs:subClassOf>
    <rdfs:label>Macroecological database of mammalian body mass Continent</rdfs:label>
    <rdfs:subClassOf rdf:resource="http://ecoinformatics.org/oboe/oboe.1.1/oboe-core.owl#MeasurementType"/>
    <rdfs:subClassOf>
      <owl:Restriction rdf:nodeID="Nb7a96ae8936243d99328adaafd38af0f">
        <owl:someValuesFrom rdf:resource="https://cn.dataone.org/cn/v2/object/doi:10.5063/AA/nceas.196.3#d_1"/>
        <owl:onProperty rdf:resource="http://ecoinformatics.org/oboe/oboe.1.1/oboe-core.owl#measuresEntity"/>
      </owl:Restriction>
    </rdfs:subClassOf>
  </owl:Class>
  <owl:Class rdf:about="https://cn.dataone.org/cn/v2/object/doi:10.5063/AA/nceas.196.3#d_2_c_1">
    <rdfs:comment>Reference number in the column Reference of the Macroecological database of mammalian body mass table.</rdfs:comment>
    <rdfs:label>Reference number</rdfs:label>
    <rdfs:subClassOf rdf:resource="http://ecoinformatics.org/oboe/oboe.1.1/oboe-core.owl#Characteristic"/>
  </owl:Class>
  <owl:Class rdf:about="https://cn.dataone.org/cn/v2/object/doi:10.5063/AA/nceas.196.3#d_1_c_1">
    <rdfs:subClassOf rdf:resource="http://ecoinformatics.org/oboe/oboe.1.1/oboe-core.owl#Characteristic"/>
    <rdfs:comment>Continent that a species resides on. If species resides on more than one continent, a continent specific body mass is reported when available. Thus, some mammals have multiple entries. The division between North and South America occurs at the isthmus of Panama.</rdfs:comment>
    <rdfs:label>Continent</rdfs:label>
  </owl:Class>
  <owl:Class rdf:about="https://cn.dataone.org/cn/v2/object/doi:10.5063/AA/nceas.196.3#d_2_c_2">
    <rdfs:label>Reference number</rdfs:label>
    <rdfs:comment>Reference number in the column Reference of the Macroecological database of mammalian body mass table.</rdfs:comment>
    <rdfs:subClassOf rdf:resource="http://ecoinformatics.org/oboe/oboe.1.1/oboe-core.owl#Characteristic"/>
  </owl:Class>
  <owl:Class rdf:about="https://cn.dataone.org/cn/v2/object/doi:10.5063/AA/nceas.196.3#d_3_c_1">
    <rdfs:label>Continental affiliations of mammals</rdfs:label>
    <rdfs:comment>Continental affiliations of mammals included in the Macroecological database of mammalian body mass.</rdfs:comment>
    <rdfs:subClassOf rdf:resource="http://ecoinformatics.org/oboe/oboe.1.1/oboe-core.owl#Characteristic"/>
  </owl:Class>
  <owl:Class rdf:about="https://cn.dataone.org/cn/v2/object/doi:10.5063/AA/nceas.196.3#d_1_c_7">
    <rdfs:subClassOf rdf:resource="http://ecoinformatics.org/oboe/oboe.1.1/oboe-core.owl#Characteristic"/>
    <rdfs:comment>Continent that a species resides on. If species resides on more than one continent, a continent specific body mass is reported when available. Thus, some mammals have multiple entries. The division between North and South America occurs at the isthmus of Panama.</rdfs:comment>
    <rdfs:label>Continent</rdfs:label>
  </owl:Class>
  <owl:Class rdf:about="https://cn.dataone.org/cn/v2/object/doi:10.5063/AA/nceas.196.3#d_1_c_4">
    <rdfs:subClassOf rdf:resource="http://ecoinformatics.org/oboe/oboe.1.1/oboe-core.owl#Characteristic"/>
    <rdfs:comment>Continent that a species resides on. If species resides on more than one continent, a continent specific body mass is reported when available. Thus, some mammals have multiple entries. The division between North and South America occurs at the isthmus of Panama.</rdfs:comment>
    <rdfs:label>Continent</rdfs:label>
  </owl:Class>
  <owl:Class rdf:about="https://cn.dataone.org/cn/v2/object/doi:10.5063/AA/nceas.196.3#d_1_c_2">
    <rdfs:label>Continent</rdfs:label>
    <rdfs:subClassOf rdf:resource="http://ecoinformatics.org/oboe/oboe.1.1/oboe-core.owl#Characteristic"/>
    <rdfs:comment>Continent that a species resides on. If species resides on more than one continent, a continent specific body mass is reported when available. Thus, some mammals have multiple entries. The division between North and South America occurs at the isthmus of Panama.</rdfs:comment>
  </owl:Class>
  <owl:Class rdf:about="https://cn.dataone.org/cn/v2/object/doi:10.5063/AA/nceas.196.3#d_1_c_6">
    <rdfs:comment>Continent that a species resides on. If species resides on more than one continent, a continent specific body mass is reported when available. Thus, some mammals have multiple entries. The division between North and South America occurs at the isthmus of Panama.</rdfs:comment>
    <rdfs:label>Continent</rdfs:label>
    <rdfs:subClassOf rdf:resource="http://ecoinformatics.org/oboe/oboe.1.1/oboe-core.owl#Characteristic"/>
  </owl:Class>
  <owl:Class rdf:about="https://cn.dataone.org/cn/v2/object/doi:10.5063/AA/nceas.196.3#d_1_c_5">
    <rdfs:subClassOf rdf:resource="http://ecoinformatics.org/oboe/oboe.1.1/oboe-core.owl#Characteristic"/>
    <rdfs:comment>Continent that a species resides on. If species resides on more than one continent, a continent specific body mass is reported when available. Thus, some mammals have multiple entries. The division between North and South America occurs at the isthmus of Panama.</rdfs:comment>
    <rdfs:label>Continent</rdfs:label>
  </owl:Class>
  <owl:Class rdf:about="https://cn.dataone.org/cn/v2/object/doi:10.5063/AA/nceas.196.3#d_1">
    <rdfs:label>Macroecological database of mammalian body mass</rdfs:label>
    <rdfs:subClassOf rdf:resource="http://ecoinformatics.org/oboe/oboe.1.1/oboe-core.owl#Entity"/>
    <rdfs:comment>Macroecological database of mammalian body mass</rdfs:comment>
  </owl:Class>
  <owl:Class rdf:about="https://cn.dataone.org/cn/v2/object/doi:10.5063/AA/nceas.196.3#d_1_c_8">
    <rdfs:comment>Continent that a species resides on. If species resides on more than one continent, a continent specific body mass is reported when available. Thus, some mammals have multiple entries. The division between North and South America occurs at the isthmus of Panama.</rdfs:comment>
    <rdfs:subClassOf rdf:resource="http://ecoinformatics.org/oboe/oboe.1.1/oboe-core.owl#Characteristic"/>
    <rdfs:label>Continent</rdfs:label>
  </owl:Class>
  <owl:Class rdf:about="https://cn.dataone.org/cn/v2/object/doi:10.5063/AA/nceas.196.3#d_3">
    <rdfs:label>Continental affiliations of mammals</rdfs:label>
    <rdfs:subClassOf rdf:resource="http://ecoinformatics.org/oboe/oboe.1.1/oboe-core.owl#Entity"/>
    <rdfs:comment>Continental affiliations of mammals included in the Macroecological database of mammalian body mass</rdfs:comment>
  </owl:Class>
  <owl:Class rdf:about="https://cn.dataone.org/cn/v2/object/doi:10.5063/AA/nceas.196.3#d_1_c_9">
    <rdfs:label>Continent</rdfs:label>
    <rdfs:subClassOf rdf:resource="http://ecoinformatics.org/oboe/oboe.1.1/oboe-core.owl#Characteristic"/>
    <rdfs:comment>Continent that a species resides on. If species resides on more than one continent, a continent specific body mass is reported when available. Thus, some mammals have multiple entries. The division between North and South America occurs at the isthmus of Panama.</rdfs:comment>
  </owl:Class>
  <owl:Class rdf:about="https://cn.dataone.org/cn/v2/object/doi:10.5063/AA/nceas.196.3#d_1_c_3">
    <rdfs:comment>Continent that a species resides on. If species resides on more than one continent, a continent specific body mass is reported when available. Thus, some mammals have multiple entries. The division between North and South America occurs at the isthmus of Panama.</rdfs:comment>
    <rdfs:label>Continent</rdfs:label>
    <rdfs:subClassOf rdf:resource="http://ecoinformatics.org/oboe/oboe.1.1/oboe-core.owl#Characteristic"/>
  </owl:Class>
  <owl:Class rdf:about="https://cn.dataone.org/cn/v2/object/doi:10.5063/AA/nceas.196.3#d_2">
    <rdfs:comment>List of citations referred to in the column Reference of the Macroecological database of mammalian body mass table</rdfs:comment>
    <rdfs:label>References</rdfs:label>
    <rdfs:subClassOf rdf:resource="http://ecoinformatics.org/oboe/oboe.1.1/oboe-core.owl#Entity"/>
  </owl:Class>
</rdf:RDF>
