<?xml version="1.0" encoding="utf-8"?>
<rdf:RDF
  xmlns:owl="http://www.w3.org/2002/07/owl#"
  xmlns:rdf="http://www.w3.org/1999/02/22-rdf-syntax-ns#"
  xmlns:rdfs="http://www.w3.org/2000/01/rdf-schema#"
>
  <owl:Class rdf:about="https://cn.dataone.org/cn/v2/object/doi:10.5063/F1B8562K#d_1_a_1">
    <rdfs:label>quadrats_2003_2004.csv </rdfs:label>
    <rdfs:subClassOf rdf:resource="http://ecoinformatics.org/oboe/oboe.1.1/oboe-core.owl#MeasurementType"/>
    <rdfs:subClassOf>
      <owl:Restriction rdf:nodeID="N31a50e8f8af943a0b6032d0b5c1b9c08">
        <owl:someValuesFrom rdf:resource="https://cn.dataone.org/cn/v2/object/doi:10.5063/F1B8562K#d_1"/>
        <owl:onProperty rdf:resource="http://ecoinformatics.org/oboe/oboe.1.1/oboe-core.owl#measuresEntity"/>
      </owl:Restriction>
    </rdfs:subClassOf>
    <rdfs:subClassOf>
      <owl:Restriction rdf:nodeID="Ndafed2ae1b00480a82811360912d61c5">
        <owl:someValuesFrom rdf:resource="https://cn.dataone.org/cn/v2/object/doi:10.5063/F1B8562K#d_1_c_1"/>
        <owl:onProperty rdf:resource="http://ecoinformatics.org/oboe/oboe.1.1/oboe-core.owl#measuresCharacteristic"/>
      </owl:Restriction>
    </rdfs:subClassOf>
  </owl:Class>
  <owl:Class rdf:about="https://cn.dataone.org/cn/v2/object/doi:10.5063/F1B8562K#d_3_a_6">
    <rdfs:subClassOf>
      <owl:Restriction rdf:nodeID="N303c99b7d81345f58a7ef0fb048b071d">
        <owl:onProperty rdf:resource="http://ecoinformatics.org/oboe/oboe.1.1/oboe-core.owl#measuresEntity"/>
        <owl:someValuesFrom rdf:resource="https://cn.dataone.org/cn/v2/object/doi:10.5063/F1B8562K#d_3"/>
      </owl:Restriction>
    </rdfs:subClassOf>
    <rdfs:label>densityMobile_2003_2004.csv </rdfs:label>
    <rdfs:subClassOf rdf:resource="http://ecoinformatics.org/oboe/oboe.1.1/oboe-core.owl#MeasurementType"/>
    <rdfs:subClassOf>
      <owl:Restriction rdf:nodeID="Naba13f84b7e14f788dfb0b6b7489f096">
        <owl:onProperty rdf:resource="http://ecoinformatics.org/oboe/oboe.1.1/oboe-core.owl#measuresCharacteristic"/>
        <owl:someValuesFrom rdf:resource="https://cn.dataone.org/cn/v2/object/doi:10.5063/F1B8562K#d_3_c_6"/>
      </owl:Restriction>
    </rdfs:subClassOf>
  </owl:Class>
  <owl:Class rdf:about="https://cn.dataone.org/cn/v2/object/doi:10.5063/F1B8562K#d_4_a_2">
    <rdfs:subClassOf>
      <owl:Restriction rdf:nodeID="N853da7a28ef34c20a50c4ed6992f9be7">
        <owl:onProperty rdf:resource="http://ecoinformatics.org/oboe/oboe.1.1/oboe-core.owl#measuresCharacteristic"/>
        <owl:someValuesFrom rdf:resource="https://cn.dataone.org/cn/v2/object/doi:10.5063/F1B8562K#d_4_c_2"/>
      </owl:Restriction>
    </rdfs:subClassOf>
    <rdfs:subClassOf rdf:resource="http://ecoinformatics.org/oboe/oboe.1.1/oboe-core.owl#MeasurementType"/>
    <rdfs:subClassOf>
      <owl:Restriction rdf:nodeID="N8fa4709ed54f4ec5b3f885c87c673af4">
        <owl:someValuesFrom rdf:resource="https://cn.dataone.org/cn/v2/object/doi:10.5063/F1B8562K#d_4"/>
        <owl:onProperty rdf:resource="http://ecoinformatics.org/oboe/oboe.1.1/oboe-core.owl#measuresEntity"/>
      </owl:Restriction>
    </rdfs:subClassOf>
    <rdfs:label>siteVisitDates_2003_2004.csv </rdfs:label>
  </owl:Class>
  <owl:Class rdf:about="https://cn.dataone.org/cn/v2/object/doi:10.5063/F1B8562K#d_1_a_5">
    <rdfs:subClassOf>
      <owl:Restriction rdf:nodeID="N4c8d0f7505ca432085945795f9c1a19c">
        <owl:someValuesFrom rdf:resource="https://cn.dataone.org/cn/v2/object/doi:10.5063/F1B8562K#d_1_c_5"/>
        <owl:onProperty rdf:resource="http://ecoinformatics.org/oboe/oboe.1.1/oboe-core.owl#measuresCharacteristic"/>
      </owl:Restriction>
    </rdfs:subClassOf>
    <rdfs:subClassOf>
      <owl:Restriction rdf:nodeID="N2551846db5ac482aa165ceb4c9a80cb1">
        <owl:someValuesFrom rdf:resource="https://cn.dataone.org/cn/v2/object/doi:10.5063/F1B8562K#d_1"/>
        <owl:onProperty rdf:resource="http://ecoinformatics.org/oboe/oboe.1.1/oboe-core.owl#measuresEntity"/>
      </owl:Restriction>
    </rdfs:subClassOf>
    <rdfs:label>quadrats_2003_2004.csv </rdfs:label>
    <rdfs:subClassOf rdf:resource="http://ecoinformatics.org/oboe/oboe.1.1/oboe-core.owl#MeasurementType"/>
  </owl:Class>
  <owl:Class rdf:about="https://cn.dataone.org/cn/v2/object/doi:10.5063/F1B8562K#d_3_a_2">
    <rdfs:label>densityMobile_2003_2004.csv </rdfs:label>
    <rdfs:subClassOf rdf:resource="http://ecoinformatics.org/oboe/oboe.1.1/oboe-core.owl#MeasurementType"/>
    <rdfs:subClassOf>
      <owl:Restriction rdf:nodeID="Nc20c3295f31c40c68eb34db58578b11f">
        <owl:onProperty rdf:resource="http://ecoinformatics.org/oboe/oboe.1.1/oboe-core.owl#measuresEntity"/>
        <owl:someValuesFrom rdf:resource="https://cn.dataone.org/cn/v2/object/doi:10.5063/F1B8562K#d_3"/>
      </owl:Restriction>
    </rdfs:subClassOf>
    <rdfs:subClassOf>
      <owl:Restriction rdf:nodeID="N12294c84ae98461b8882252f10ad8ae0">
        <owl:onProperty rdf:resource="http://ecoinformatics.org/oboe/oboe.1.1/oboe-core.owl#measuresCharacteristic"/>
        <owl:someValuesFrom rdf:resource="https://cn.dataone.org/cn/v2/object/doi:10.5063/F1B8562K#d_3_c_2"/>
      </owl:Restriction>
    </rdfs:subClassOf>
  </owl:Class>
  <owl:Class rdf:about="https://cn.dataone.org/cn/v2/object/doi:10.5063/F1B8562K#d_3_a_3">
    <rdfs:subClassOf>
      <owl:Restriction rdf:nodeID="N29376e1e2c644b1a9abb630526aba1c0">
        <owl:onProperty rdf:resource="http://ecoinformatics.org/oboe/oboe.1.1/oboe-core.owl#measuresEntity"/>
        <owl:someValuesFrom rdf:resource="https://cn.dataone.org/cn/v2/object/doi:10.5063/F1B8562K#d_3"/>
      </owl:Restriction>
    </rdfs:subClassOf>
    <rdfs:subClassOf>
      <owl:Restriction rdf:nodeID="Na69714de8269485a9fb59d0882f36d57">
        <owl:onProperty rdf:resource="http://ecoinformatics.org/oboe/oboe.1.1/oboe-core.owl#measuresCharacteristic"/>
        <owl:someValuesFrom rdf:resource="https://cn.dataone.org/cn/v2/object/doi:10.5063/F1B8562K#d_3_c_3"/>
      </owl:Restriction>
    </rdfs:subClassOf>
    <rdfs:subClassOf rdf:resource="http://ecoinformatics.org/oboe/oboe.1.1/oboe-core.owl#MeasurementType"/>
    <rdfs:label>densityMobile_2003_2004.csv </rdfs:label>
  </owl:Class>
  <owl:Class rdf:about="https://cn.dataone.org/cn/v2/object/doi:10.5063/F1B8562K#d_1_a_2">
    <rdfs:label>quadrats_2003_2004.csv </rdfs:label>
    <rdfs:subClassOf>
      <owl:Restriction rdf:nodeID="Nb990fd79bd4c4ef2a5363d166aac3234">
        <owl:onProperty rdf:resource="http://ecoinformatics.org/oboe/oboe.1.1/oboe-core.owl#measuresEntity"/>
        <owl:someValuesFrom rdf:resource="https://cn.dataone.org/cn/v2/object/doi:10.5063/F1B8562K#d_1"/>
      </owl:Restriction>
    </rdfs:subClassOf>
    <rdfs:subClassOf rdf:resource="http://ecoinformatics.org/oboe/oboe.1.1/oboe-core.owl#MeasurementType"/>
    <rdfs:subClassOf>
      <owl:Restriction rdf:nodeID="N418a5f3a20f643139590ff9616c0f649">
        <owl:someValuesFrom rdf:resource="https://cn.dataone.org/cn/v2/object/doi:10.5063/F1B8562K#d_1_c_2"/>
        <owl:onProperty rdf:resource="http://ecoinformatics.org/oboe/oboe.1.1/oboe-core.owl#measuresCharacteristic"/>
      </owl:Restriction>
    </rdfs:subClassOf>
  </owl:Class>
  <owl:Class rdf:about="https://cn.dataone.org/cn/v2/object/doi:10.5063/F1B8562K#d_3_a_1">
    <rdfs:label>densityMobile_2003_2004.csv </rdfs:label>
    <rdfs:subClassOf rdf:resource="http://ecoinformatics.org/oboe/oboe.1.1/oboe-core.owl#MeasurementType"/>
    <rdfs:subClassOf>
      <owl:Restriction rdf:nodeID="N40a95aecd7a54ce7842081c5261e4ae7">
        <owl:onProperty rdf:resource="http://ecoinformatics.org/oboe/oboe.1.1/oboe-core.owl#measuresEntity"/>
        <owl:someValuesFrom rdf:resource="https://cn.dataone.org/cn/v2/object/doi:10.5063/F1B8562K#d_3"/>
      </owl:Restriction>
    </rdfs:subClassOf>
    <rdfs:subClassOf>
      <owl:Restriction rdf:nodeID="Ne8fc11e4eb3d4c0dbfe07ba235121169">
        <owl:onProperty rdf:resource="http://ecoinformatics.org/oboe/oboe.1.1/oboe-core.owl#measuresCharacteristic"/>
        <owl:someValuesFrom rdf:resource="https://cn.dataone.org/cn/v2/object/doi:10.5063/F1B8562K#d_3_c_1"/>
      </owl:Restriction>
    </rdfs:subClassOf>
  </owl:Class>
  <owl:Class rdf:about="https://cn.dataone.org/cn/v2/object/doi:10.5063/F1B8562K#d_2_a_1">
    <rdfs:subClassOf>
      <owl:Restriction rdf:nodeID="Nfad0958836d542328266d5220f58f7ba">
        <owl:onProperty rdf:resource="http://ecoinformatics.org/oboe/oboe.1.1/oboe-core.owl#measuresEntity"/>
        <owl:someValuesFrom rdf:resource="https://cn.dataone.org/cn/v2/object/doi:10.5063/F1B8562K#d_2"/>
      </owl:Restriction>
    </rdfs:subClassOf>
    <rdfs:label>percentCoverSessile_2003_2004.csv </rdfs:label>
    <rdfs:subClassOf rdf:resource="http://ecoinformatics.org/oboe/oboe.1.1/oboe-core.owl#MeasurementType"/>
    <rdfs:subClassOf>
      <owl:Restriction rdf:nodeID="Ncd2ea5f2d9704677a77c6352d4f424d6">
        <owl:onProperty rdf:resource="http://ecoinformatics.org/oboe/oboe.1.1/oboe-core.owl#measuresCharacteristic"/>
        <owl:someValuesFrom rdf:resource="https://cn.dataone.org/cn/v2/object/doi:10.5063/F1B8562K#d_2_c_1"/>
      </owl:Restriction>
    </rdfs:subClassOf>
  </owl:Class>
  <owl:Class rdf:about="https://cn.dataone.org/cn/v2/object/doi:10.5063/F1B8562K#d_2_a_5">
    <rdfs:subClassOf>
      <owl:Restriction rdf:nodeID="N2d2ffc746ba24c1d926aef9fff4a118f">
        <owl:onProperty rdf:resource="http://ecoinformatics.org/oboe/oboe.1.1/oboe-core.owl#measuresEntity"/>
        <owl:someValuesFrom rdf:resource="https://cn.dataone.org/cn/v2/object/doi:10.5063/F1B8562K#d_2"/>
      </owl:Restriction>
    </rdfs:subClassOf>
    <rdfs:label>percentCoverSessile_2003_2004.csv </rdfs:label>
    <rdfs:subClassOf rdf:resource="http://ecoinformatics.org/oboe/oboe.1.1/oboe-core.owl#MeasurementType"/>
    <rdfs:subClassOf>
      <owl:Restriction rdf:nodeID="N2ab742a5ccfd404691f29da126641d31">
        <owl:someValuesFrom rdf:resource="https://cn.dataone.org/cn/v2/object/doi:10.5063/F1B8562K#d_2_c_5"/>
        <owl:onProperty rdf:resource="http://ecoinformatics.org/oboe/oboe.1.1/oboe-core.owl#measuresCharacteristic"/>
      </owl:Restriction>
    </rdfs:subClassOf>
  </owl:Class>
  <owl:Class rdf:about="https://cn.dataone.org/cn/v2/object/doi:10.5063/F1B8562K#d_4_a_1">
    <rdfs:subClassOf rdf:resource="http://ecoinformatics.org/oboe/oboe.1.1/oboe-core.owl#MeasurementType"/>
    <rdfs:label>siteVisitDates_2003_2004.csv </rdfs:label>
    <rdfs:subClassOf>
      <owl:Restriction rdf:nodeID="Na384e0d3c4dd4ccebf458a8fded62bfe">
        <owl:someValuesFrom rdf:resource="https://cn.dataone.org/cn/v2/object/doi:10.5063/F1B8562K#d_4_c_1"/>
        <owl:onProperty rdf:resource="http://ecoinformatics.org/oboe/oboe.1.1/oboe-core.owl#measuresCharacteristic"/>
      </owl:Restriction>
    </rdfs:subClassOf>
    <rdfs:subClassOf>
      <owl:Restriction rdf:nodeID="N5454394875054f1abb6df835e5b16a96">
        <owl:onProperty rdf:resource="http://ecoinformatics.org/oboe/oboe.1.1/oboe-core.owl#measuresEntity"/>
        <owl:someValuesFrom rdf:resource="https://cn.dataone.org/cn/v2/object/doi:10.5063/F1B8562K#d_4"/>
      </owl:Restriction>
    </rdfs:subClassOf>
  </owl:Class>
  <owl:Class rdf:about="https://cn.dataone.org/cn/v2/object/doi:10.5063/F1B8562K#d_2_a_4">
    <rdfs:subClassOf rdf:resource="http://ecoinformatics.org/oboe/oboe.1.1/oboe-core.owl#MeasurementType"/>
    <rdfs:subClassOf>
      <owl:Restriction rdf:nodeID="N9ce275649bd2428e8397809e1476514a">
        <owl:onProperty rdf:resource="http://ecoinformatics.org/oboe/oboe.1.1/oboe-core.owl#measuresEntity"/>
        <owl:someValuesFrom rdf:resource="https://cn.dataone.org/cn/v2/object/doi:10.5063/F1B8562K#d_2"/>
      </owl:Restriction>
    </rdfs:subClassOf>
    <rdfs:label>percentCoverSessile_2003_2004.csv </rdfs:label>
    <rdfs:subClassOf>
      <owl:Restriction rdf:nodeID="Nad46e3036c674890ab8bc86decd604ee">
        <owl:someValuesFrom rdf:resource="https://cn.dataone.org/cn/v2/object/doi:10.5063/F1B8562K#d_2_c_4"/>
        <owl:onProperty rdf:resource="http://ecoinformatics.org/oboe/oboe.1.1/oboe-core.owl#measuresCharacteristic"/>
      </owl:Restriction>
    </rdfs:subClassOf>
  </owl:Class>
  <owl:Class rdf:about="https://cn.dataone.org/cn/v2/object/doi:10.5063/F1B8562K#d_1_a_3">
    <rdfs:label>quadrats_2003_2004.csv </rdfs:label>
    <rdfs:subClassOf>
      <owl:Restriction rdf:nodeID="Nd83165f287014c5ca4181beefaede1c4">
        <owl:someValuesFrom rdf:resource="https://cn.dataone.org/cn/v2/object/doi:10.5063/F1B8562K#d_1"/>
        <owl:onProperty rdf:resource="http://ecoinformatics.org/oboe/oboe.1.1/oboe-core.owl#measuresEntity"/>
      </owl:Restriction>
    </rdfs:subClassOf>
    <rdfs:subClassOf rdf:resource="http://ecoinformatics.org/oboe/oboe.1.1/oboe-core.owl#MeasurementType"/>
    <rdfs:subClassOf>
      <owl:Restriction rdf:nodeID="N4837f821991546999659a083cafbd54f">
        <owl:someValuesFrom rdf:resource="https://cn.dataone.org/cn/v2/object/doi:10.5063/F1B8562K#d_1_c_3"/>
        <owl:onProperty rdf:resource="http://ecoinformatics.org/oboe/oboe.1.1/oboe-core.owl#measuresCharacteristic"/>
      </owl:Restriction>
    </rdfs:subClassOf>
  </owl:Class>
  <owl:Class rdf:about="https://cn.dataone.org/cn/v2/object/doi:10.5063/F1B8562K#d_1_a_6">
    <rdfs:label>quadrats_2003_2004.csv </rdfs:label>
    <rdfs:subClassOf>
      <owl:Restriction rdf:nodeID="N38c6c9d0d5174358b4ae42079c84e6f5">
        <owl:someValuesFrom rdf:resource="https://cn.dataone.org/cn/v2/object/doi:10.5063/F1B8562K#d_1_c_6"/>
        <owl:onProperty rdf:resource="http://ecoinformatics.org/oboe/oboe.1.1/oboe-core.owl#measuresCharacteristic"/>
      </owl:Restriction>
    </rdfs:subClassOf>
    <rdfs:subClassOf rdf:resource="http://ecoinformatics.org/oboe/oboe.1.1/oboe-core.owl#MeasurementType"/>
    <rdfs:subClassOf>
      <owl:Restriction rdf:nodeID="N47b2796603914840a8e95281e68d3c31">
        <owl:someValuesFrom rdf:resource="https://cn.dataone.org/cn/v2/object/doi:10.5063/F1B8562K#d_1"/>
        <owl:onProperty rdf:resource="http://ecoinformatics.org/oboe/oboe.1.1/oboe-core.owl#measuresEntity"/>
      </owl:Restriction>
    </rdfs:subClassOf>
  </owl:Class>
  <owl:Class rdf:about="https://cn.dataone.org/cn/v2/object/doi:10.5063/F1B8562K#d_4_a_3">
    <rdfs:subClassOf rdf:resource="http://ecoinformatics.org/oboe/oboe.1.1/oboe-core.owl#MeasurementType"/>
    <rdfs:label>siteVisitDates_2003_2004.csv </rdfs:label>
    <rdfs:subClassOf>
      <owl:Restriction rdf:nodeID="N907fe39e16fc4ade93db46cddb8cc8e6">
        <owl:onProperty rdf:resource="http://ecoinformatics.org/oboe/oboe.1.1/oboe-core.owl#measuresEntity"/>
        <owl:someValuesFrom rdf:resource="https://cn.dataone.org/cn/v2/object/doi:10.5063/F1B8562K#d_4"/>
      </owl:Restriction>
    </rdfs:subClassOf>
    <rdfs:subClassOf>
      <owl:Restriction rdf:nodeID="Nf51c9834ea1e449495ae24741d32366e">
        <owl:onProperty rdf:resource="http://ecoinformatics.org/oboe/oboe.1.1/oboe-core.owl#measuresCharacteristic"/>
        <owl:someValuesFrom rdf:resource="https://cn.dataone.org/cn/v2/object/doi:10.5063/F1B8562K#d_4_c_3"/>
      </owl:Restriction>
    </rdfs:subClassOf>
  </owl:Class>
  <owl:Class rdf:about="https://cn.dataone.org/cn/v2/object/doi:10.5063/F1B8562K#d_2_a_2">
    <rdfs:label>percentCoverSessile_2003_2004.csv </rdfs:label>
    <rdfs:subClassOf>
      <owl:Restriction rdf:nodeID="Na101b6f7308b40f1b3be83a6c62cd23f">
        <owl:onProperty rdf:resource="http://ecoinformatics.org/oboe/oboe.1.1/oboe-core.owl#measuresEntity"/>
        <owl:someValuesFrom rdf:resource="https://cn.dataone.org/cn/v2/object/doi:10.5063/F1B8562K#d_2"/>
      </owl:Restriction>
    </rdfs:subClassOf>
    <rdfs:subClassOf>
      <owl:Restriction rdf:nodeID="N36d7e3c67e254c80abe4b596fe335ea1">
        <owl:onProperty rdf:resource="http://ecoinformatics.org/oboe/oboe.1.1/oboe-core.owl#measuresCharacteristic"/>
        <owl:someValuesFrom rdf:resource="https://cn.dataone.org/cn/v2/object/doi:10.5063/F1B8562K#d_2_c_2"/>
      </owl:Restriction>
    </rdfs:subClassOf>
    <rdfs:subClassOf rdf:resource="http://ecoinformatics.org/oboe/oboe.1.1/oboe-core.owl#MeasurementType"/>
  </owl:Class>
  <owl:Class rdf:about="https://cn.dataone.org/cn/v2/object/doi:10.5063/F1B8562K#d_1_a_7">
    <rdfs:subClassOf>
      <owl:Restriction rdf:nodeID="N3d77090e7835445e802c5701aff7ab1a">
        <owl:onProperty rdf:resource="http://ecoinformatics.org/oboe/oboe.1.1/oboe-core.owl#measuresEntity"/>
        <owl:someValuesFrom rdf:resource="https://cn.dataone.org/cn/v2/object/doi:10.5063/F1B8562K#d_1"/>
      </owl:Restriction>
    </rdfs:subClassOf>
    <rdfs:label>quadrats_2003_2004.csv </rdfs:label>
    <rdfs:subClassOf rdf:resource="http://ecoinformatics.org/oboe/oboe.1.1/oboe-core.owl#MeasurementType"/>
    <rdfs:subClassOf>
      <owl:Restriction rdf:nodeID="Nebdf6d36b22d4ee68c46f7a32d9439ad">
        <owl:onProperty rdf:resource="http://ecoinformatics.org/oboe/oboe.1.1/oboe-core.owl#measuresCharacteristic"/>
        <owl:someValuesFrom rdf:resource="https://cn.dataone.org/cn/v2/object/doi:10.5063/F1B8562K#d_1_c_7"/>
      </owl:Restriction>
    </rdfs:subClassOf>
  </owl:Class>
  <owl:Class rdf:about="https://cn.dataone.org/cn/v2/object/doi:10.5063/F1B8562K#d_1_a_4">
    <rdfs:subClassOf rdf:resource="http://ecoinformatics.org/oboe/oboe.1.1/oboe-core.owl#MeasurementType"/>
    <rdfs:subClassOf>
      <owl:Restriction rdf:nodeID="N9ca4d35d962d461287b3979a5df939a5">
        <owl:someValuesFrom rdf:resource="https://cn.dataone.org/cn/v2/object/doi:10.5063/F1B8562K#d_1"/>
        <owl:onProperty rdf:resource="http://ecoinformatics.org/oboe/oboe.1.1/oboe-core.owl#measuresEntity"/>
      </owl:Restriction>
    </rdfs:subClassOf>
    <rdfs:label>quadrats_2003_2004.csv </rdfs:label>
    <rdfs:subClassOf>
      <owl:Restriction rdf:nodeID="Nd677cfd338c64ff2ba31e9a35cedb903">
        <owl:onProperty rdf:resource="http://ecoinformatics.org/oboe/oboe.1.1/oboe-core.owl#measuresCharacteristic"/>
        <owl:someValuesFrom rdf:resource="https://cn.dataone.org/cn/v2/object/doi:10.5063/F1B8562K#d_1_c_4"/>
      </owl:Restriction>
    </rdfs:subClassOf>
  </owl:Class>
  <owl:Class rdf:about="https://cn.dataone.org/cn/v2/object/doi:10.5063/F1B8562K#d_3_a_5">
    <rdfs:subClassOf>
      <owl:Restriction rdf:nodeID="Nc8afa41b8f214665903b483cb918ba90">
        <owl:onProperty rdf:resource="http://ecoinformatics.org/oboe/oboe.1.1/oboe-core.owl#measuresEntity"/>
        <owl:someValuesFrom rdf:resource="https://cn.dataone.org/cn/v2/object/doi:10.5063/F1B8562K#d_3"/>
      </owl:Restriction>
    </rdfs:subClassOf>
    <rdfs:subClassOf>
      <owl:Restriction rdf:nodeID="Nce214e5089ff45a9b9911361d11cc3b1">
        <owl:someValuesFrom rdf:resource="https://cn.dataone.org/cn/v2/object/doi:10.5063/F1B8562K#d_3_c_5"/>
        <owl:onProperty rdf:resource="http://ecoinformatics.org/oboe/oboe.1.1/oboe-core.owl#measuresCharacteristic"/>
      </owl:Restriction>
    </rdfs:subClassOf>
    <rdfs:subClassOf rdf:resource="http://ecoinformatics.org/oboe/oboe.1.1/oboe-core.owl#MeasurementType"/>
    <rdfs:label>densityMobile_2003_2004.csv </rdfs:label>
  </owl:Class>
  <owl:Class rdf:about="https://cn.dataone.org/cn/v2/object/doi:10.5063/F1B8562K#d_2_a_6">
    <rdfs:subClassOf rdf:resource="http://ecoinformatics.org/oboe/oboe.1.1/oboe-core.owl#MeasurementType"/>
    <rdfs:subClassOf>
      <owl:Restriction rdf:nodeID="N127f3d6c483449c3a2b6385d428ac096">
        <owl:onProperty rdf:resource="http://ecoinformatics.org/oboe/oboe.1.1/oboe-core.owl#measuresEntity"/>
        <owl:someValuesFrom rdf:resource="https://cn.dataone.org/cn/v2/object/doi:10.5063/F1B8562K#d_2"/>
      </owl:Restriction>
    </rdfs:subClassOf>
    <rdfs:subClassOf>
      <owl:Restriction rdf:nodeID="Nef81ebb0216844deabc8fbb72b56a8a6">
        <owl:onProperty rdf:resource="http://ecoinformatics.org/oboe/oboe.1.1/oboe-core.owl#measuresCharacteristic"/>
        <owl:someValuesFrom rdf:resource="https://cn.dataone.org/cn/v2/object/doi:10.5063/F1B8562K#d_2_c_6"/>
      </owl:Restriction>
    </rdfs:subClassOf>
    <rdfs:label>percentCoverSessile_2003_2004.csv </rdfs:label>
  </owl:Class>
  <owl:Class rdf:about="https://cn.dataone.org/cn/v2/object/doi:10.5063/F1B8562K#d_1_a_8">
    <rdfs:subClassOf rdf:resource="http://ecoinformatics.org/oboe/oboe.1.1/oboe-core.owl#MeasurementType"/>
    <rdfs:label>quadrats_2003_2004.csv </rdfs:label>
    <rdfs:subClassOf>
      <owl:Restriction rdf:nodeID="N97f4e42db263442d96713ffb82118f95">
        <owl:onProperty rdf:resource="http://ecoinformatics.org/oboe/oboe.1.1/oboe-core.owl#measuresCharacteristic"/>
        <owl:someValuesFrom rdf:resource="https://cn.dataone.org/cn/v2/object/doi:10.5063/F1B8562K#d_1_c_8"/>
      </owl:Restriction>
    </rdfs:subClassOf>
    <rdfs:subClassOf>
      <owl:Restriction rdf:nodeID="N65a8c85cab78487a837a9aa3309ea00a">
        <owl:someValuesFrom rdf:resource="https://cn.dataone.org/cn/v2/object/doi:10.5063/F1B8562K#d_1"/>
        <owl:onProperty rdf:resource="http://ecoinformatics.org/oboe/oboe.1.1/oboe-core.owl#measuresEntity"/>
      </owl:Restriction>
    </rdfs:subClassOf>
  </owl:Class>
  <owl:Class rdf:about="https://cn.dataone.org/cn/v2/object/doi:10.5063/F1B8562K#d_3_a_4">
    <rdfs:label>densityMobile_2003_2004.csv </rdfs:label>
    <rdfs:subClassOf rdf:resource="http://ecoinformatics.org/oboe/oboe.1.1/oboe-core.owl#MeasurementType"/>
    <rdfs:subClassOf>
      <owl:Restriction rdf:nodeID="N1ed2f6d839e944429e6205d94733f1ab">
        <owl:someValuesFrom rdf:resource="https://cn.dataone.org/cn/v2/object/doi:10.5063/F1B8562K#d_3_c_4"/>
        <owl:onProperty rdf:resource="http://ecoinformatics.org/oboe/oboe.1.1/oboe-core.owl#measuresCharacteristic"/>
      </owl:Restriction>
    </rdfs:subClassOf>
    <rdfs:subClassOf>
      <owl:Restriction rdf:nodeID="N15ddf382b4cb49768192ff9ecb08d193">
        <owl:onProperty rdf:resource="http://ecoinformatics.org/oboe/oboe.1.1/oboe-core.owl#measuresEntity"/>
        <owl:someValuesFrom rdf:resource="https://cn.dataone.org/cn/v2/object/doi:10.5063/F1B8562K#d_3"/>
      </owl:Restriction>
    </rdfs:subClassOf>
  </owl:Class>
  <owl:Class rdf:about="https://cn.dataone.org/cn/v2/object/doi:10.5063/F1B8562K#d_2_a_3">
    <rdfs:label>percentCoverSessile_2003_2004.csv </rdfs:label>
    <rdfs:subClassOf rdf:resource="http://ecoinformatics.org/oboe/oboe.1.1/oboe-core.owl#MeasurementType"/>
    <rdfs:subClassOf>
      <owl:Restriction rdf:nodeID="Na9b4c81361c44e6282b34428b6525025">
        <owl:onProperty rdf:resource="http://ecoinformatics.org/oboe/oboe.1.1/oboe-core.owl#measuresEntity"/>
        <owl:someValuesFrom rdf:resource="https://cn.dataone.org/cn/v2/object/doi:10.5063/F1B8562K#d_2"/>
      </owl:Restriction>
    </rdfs:subClassOf>
    <rdfs:subClassOf>
      <owl:Restriction rdf:nodeID="N229daf827f5e428da0db7d34d70773a1">
        <owl:onProperty rdf:resource="http://ecoinformatics.org/oboe/oboe.1.1/oboe-core.owl#measuresCharacteristic"/>
        <owl:someValuesFrom rdf:resource="https://cn.dataone.org/cn/v2/object/doi:10.5063/F1B8562K#d_2_c_3"/>
      </owl:Restriction>
    </rdfs:subClassOf>
  </owl:Class>
  <owl:Ontology rdf:about="https://cn.dataone.org/cn/v2/object/doi:10.5063/F1B8562K">
    <rdfs:comment>We investigated the relative roles of natural factors and shoreline harvest leading to localized declines of the black leather chiton, Katharina tunicata, on the Kenai Peninsula, Alaska. Field surveys of the significant predictors of K. tunicata across 11 sites suggest that its current spatial variation is significantly related to human exploitation and sea otter predation. Traditional ecological knowledge further revealed that several benthic marine invertebrates (sea urchin, crab and clams) have declined sequentially, with reduced densities of K. tunicata being the most recent. We propose that a restriction in alternative prey species availability has led to recent intensified per capita predator impacts on K. tunicata. Experimental K. tunicata removals in the low intertidal revealed that at high densities, K. tunicata reduced the density of Alaria marginata, by 94% and species richness by 38%, and altered algal and invertebrate community structure. Across site comparisons showed that A. marginata biomass was 7 times greater at exploited versus unexploited sites. Furthermore, community structure differed significantly as a function of predation pressure. These results provide evidence of a trophic cascade and reveal the extent to which fishing and natural predation, via the reduction of a shared keystone resource, indirectly alter a temperate coastal ecosystem. 

Publications: 
Salomon, A.K. 2006. Investigating the relative roles of natural factors and shoreline harvest in altering the community structure, dynamics and diversity of the Kenai Peninsula's rocky intertidal, Exxon Valdez Oil Spill Gulf Ecosystem Monitoring and Research Project Final Report (GEM Project 030647), University of Washington, Seattle, Washington.</rdfs:comment>
    <rdfs:label>Rocky intertidal species diversity along the Kenai Peninsula, Alaska: 2003 - 2004</rdfs:label>
  </owl:Ontology>
  <owl:Class rdf:about="https://cn.dataone.org/cn/v2/object/doi:10.5063/F1B8562K#d_2">
    <rdfs:label>percentCoverSessile_2003_2004.csv</rdfs:label>
    <rdfs:subClassOf rdf:resource="http://ecoinformatics.org/oboe/oboe.1.1/oboe-core.owl#Entity"/>
    <rdfs:comment>Percent cover estimates for algae and sessile invertebrates in quadrats at 11 sample sites, 2003 and 2004.</rdfs:comment>
  </owl:Class>
  <owl:Class rdf:about="https://cn.dataone.org/cn/v2/object/doi:10.5063/F1B8562K#d_1_c_8">
    <rdfs:subClassOf rdf:resource="http://ecoinformatics.org/oboe/oboe.1.1/oboe-core.owl#Characteristic"/>
    <rdfs:comment>Sample site name, 11 sites total. Unsure what the 'Liz Quad' stands for in some site names.</rdfs:comment>
  </owl:Class>
  <owl:Class rdf:about="https://cn.dataone.org/cn/v2/object/doi:10.5063/F1B8562K#d_3_c_5">
    <rdfs:comment>Date of quadrat sampling where known. Four digit year is put where no date could be found, but may be able to corrobrate with 'dateVisits.csv' table. Unsure what 'not so good' stands for.</rdfs:comment>
    <rdfs:subClassOf rdf:resource="http://ecoinformatics.org/oboe/oboe.1.1/oboe-core.owl#Characteristic"/>
  </owl:Class>
  <owl:Class rdf:about="https://cn.dataone.org/cn/v2/object/doi:10.5063/F1B8562K#d_3_c_6">
    <rdfs:subClassOf rdf:resource="http://ecoinformatics.org/oboe/oboe.1.1/oboe-core.owl#Characteristic"/>
    <rdfs:comment>Date of quadrat sampling where known. Four digit year is put where no date could be found, but may be able to corrobrate with 'dateVisits.csv' table. Unsure what 'not so good' stands for.</rdfs:comment>
  </owl:Class>
  <owl:Class rdf:about="https://cn.dataone.org/cn/v2/object/doi:10.5063/F1B8562K#d_3">
    <rdfs:subClassOf rdf:resource="http://ecoinformatics.org/oboe/oboe.1.1/oboe-core.owl#Entity"/>
    <rdfs:label>densityMobile_2003_2004.csv</rdfs:label>
    <rdfs:comment>Counts of mobile invertebrates in quadrats at 11 sample sites, 2003 and 2004.</rdfs:comment>
  </owl:Class>
  <owl:Class rdf:about="https://cn.dataone.org/cn/v2/object/doi:10.5063/F1B8562K#d_3_c_1">
    <rdfs:subClassOf rdf:resource="http://ecoinformatics.org/oboe/oboe.1.1/oboe-core.owl#Characteristic"/>
    <rdfs:comment>Date of quadrat sampling where known. Four digit year is put where no date could be found, but may be able to corrobrate with 'dateVisits.csv' table. Unsure what 'not so good' stands for.</rdfs:comment>
  </owl:Class>
  <owl:Class rdf:about="https://cn.dataone.org/cn/v2/object/doi:10.5063/F1B8562K#d_4_c_3">
    <rdfs:comment>Sample site name, 11 sites total.</rdfs:comment>
    <rdfs:subClassOf rdf:resource="http://ecoinformatics.org/oboe/oboe.1.1/oboe-core.owl#Characteristic"/>
  </owl:Class>
  <owl:Class rdf:about="https://cn.dataone.org/cn/v2/object/doi:10.5063/F1B8562K#d_1">
    <rdfs:subClassOf rdf:resource="http://ecoinformatics.org/oboe/oboe.1.1/oboe-core.owl#Entity"/>
    <rdfs:comment>Length and sometimes the derived biomass for snails, algae and katharina tunicata at 11 sample sites, 2003 and 2004.</rdfs:comment>
    <rdfs:label>quadrats_2003_2004.csv</rdfs:label>
  </owl:Class>
  <owl:Class rdf:about="https://cn.dataone.org/cn/v2/object/doi:10.5063/F1B8562K#d_4">
    <rdfs:comment>Improvised table attempting to aggregate all site visit dates</rdfs:comment>
    <rdfs:subClassOf rdf:resource="http://ecoinformatics.org/oboe/oboe.1.1/oboe-core.owl#Entity"/>
    <rdfs:label>siteVisitDates_2003_2004.csv</rdfs:label>
  </owl:Class>
  <owl:Class rdf:about="https://cn.dataone.org/cn/v2/object/doi:10.5063/F1B8562K#d_4_c_2">
    <rdfs:comment>Sample site name, 11 sites total.</rdfs:comment>
    <rdfs:subClassOf rdf:resource="http://ecoinformatics.org/oboe/oboe.1.1/oboe-core.owl#Characteristic"/>
  </owl:Class>
  <owl:Class rdf:about="https://cn.dataone.org/cn/v2/object/doi:10.5063/F1B8562K#d_4_c_1">
    <rdfs:comment>Sample site name, 11 sites total.</rdfs:comment>
    <rdfs:subClassOf rdf:resource="http://ecoinformatics.org/oboe/oboe.1.1/oboe-core.owl#Characteristic"/>
  </owl:Class>
  <owl:Class rdf:about="https://cn.dataone.org/cn/v2/object/doi:10.5063/F1B8562K#d_1_c_5">
    <rdfs:comment>Sample site name, 11 sites total. Unsure what the 'Liz Quad' stands for in some site names.</rdfs:comment>
    <rdfs:subClassOf rdf:resource="http://ecoinformatics.org/oboe/oboe.1.1/oboe-core.owl#Characteristic"/>
  </owl:Class>
  <owl:Class rdf:about="https://cn.dataone.org/cn/v2/object/doi:10.5063/F1B8562K#d_2_c_1">
    <rdfs:subClassOf rdf:resource="http://ecoinformatics.org/oboe/oboe.1.1/oboe-core.owl#Characteristic"/>
    <rdfs:comment>Date of quadrat sampling where known. Four digit year is put where no date could be found, but may be able to corrobrate with 'dateVisits.csv' table. Unsure what 'not so good' stands for.</rdfs:comment>
  </owl:Class>
  <owl:Class rdf:about="https://cn.dataone.org/cn/v2/object/doi:10.5063/F1B8562K#d_1_c_2">
    <rdfs:subClassOf rdf:resource="http://ecoinformatics.org/oboe/oboe.1.1/oboe-core.owl#Characteristic"/>
    <rdfs:comment>Sample site name, 11 sites total. Unsure what the 'Liz Quad' stands for in some site names.</rdfs:comment>
  </owl:Class>
  <owl:Class rdf:about="https://cn.dataone.org/cn/v2/object/doi:10.5063/F1B8562K#d_2_c_4">
    <rdfs:subClassOf rdf:resource="http://ecoinformatics.org/oboe/oboe.1.1/oboe-core.owl#Characteristic"/>
    <rdfs:comment>Date of quadrat sampling where known. Four digit year is put where no date could be found, but may be able to corrobrate with 'dateVisits.csv' table. Unsure what 'not so good' stands for.</rdfs:comment>
  </owl:Class>
  <owl:Class rdf:about="https://cn.dataone.org/cn/v2/object/doi:10.5063/F1B8562K#d_2_c_2">
    <rdfs:subClassOf rdf:resource="http://ecoinformatics.org/oboe/oboe.1.1/oboe-core.owl#Characteristic"/>
    <rdfs:comment>Date of quadrat sampling where known. Four digit year is put where no date could be found, but may be able to corrobrate with 'dateVisits.csv' table. Unsure what 'not so good' stands for.</rdfs:comment>
  </owl:Class>
  <owl:Class rdf:about="https://cn.dataone.org/cn/v2/object/doi:10.5063/F1B8562K#d_1_c_6">
    <rdfs:subClassOf rdf:resource="http://ecoinformatics.org/oboe/oboe.1.1/oboe-core.owl#Characteristic"/>
    <rdfs:comment>Sample site name, 11 sites total. Unsure what the 'Liz Quad' stands for in some site names.</rdfs:comment>
  </owl:Class>
  <owl:Class rdf:about="https://cn.dataone.org/cn/v2/object/doi:10.5063/F1B8562K#d_3_c_4">
    <rdfs:comment>Date of quadrat sampling where known. Four digit year is put where no date could be found, but may be able to corrobrate with 'dateVisits.csv' table. Unsure what 'not so good' stands for.</rdfs:comment>
    <rdfs:subClassOf rdf:resource="http://ecoinformatics.org/oboe/oboe.1.1/oboe-core.owl#Characteristic"/>
  </owl:Class>
  <owl:Class rdf:about="https://cn.dataone.org/cn/v2/object/doi:10.5063/F1B8562K#d_3_c_3">
    <rdfs:subClassOf rdf:resource="http://ecoinformatics.org/oboe/oboe.1.1/oboe-core.owl#Characteristic"/>
    <rdfs:comment>Date of quadrat sampling where known. Four digit year is put where no date could be found, but may be able to corrobrate with 'dateVisits.csv' table. Unsure what 'not so good' stands for.</rdfs:comment>
  </owl:Class>
  <owl:Class rdf:about="https://cn.dataone.org/cn/v2/object/doi:10.5063/F1B8562K#d_2_c_6">
    <rdfs:comment>Date of quadrat sampling where known. Four digit year is put where no date could be found, but may be able to corrobrate with 'dateVisits.csv' table. Unsure what 'not so good' stands for.</rdfs:comment>
    <rdfs:subClassOf rdf:resource="http://ecoinformatics.org/oboe/oboe.1.1/oboe-core.owl#Characteristic"/>
  </owl:Class>
  <owl:Class rdf:about="https://cn.dataone.org/cn/v2/object/doi:10.5063/F1B8562K#d_1_c_7">
    <rdfs:subClassOf rdf:resource="http://ecoinformatics.org/oboe/oboe.1.1/oboe-core.owl#Characteristic"/>
    <rdfs:comment>Sample site name, 11 sites total. Unsure what the 'Liz Quad' stands for in some site names.</rdfs:comment>
  </owl:Class>
  <owl:Class rdf:about="https://cn.dataone.org/cn/v2/object/doi:10.5063/F1B8562K#d_3_c_2">
    <rdfs:comment>Date of quadrat sampling where known. Four digit year is put where no date could be found, but may be able to corrobrate with 'dateVisits.csv' table. Unsure what 'not so good' stands for.</rdfs:comment>
    <rdfs:subClassOf rdf:resource="http://ecoinformatics.org/oboe/oboe.1.1/oboe-core.owl#Characteristic"/>
  </owl:Class>
  <owl:Class rdf:about="https://cn.dataone.org/cn/v2/object/doi:10.5063/F1B8562K#d_1_c_4">
    <rdfs:subClassOf rdf:resource="http://ecoinformatics.org/oboe/oboe.1.1/oboe-core.owl#Characteristic"/>
    <rdfs:comment>Sample site name, 11 sites total. Unsure what the 'Liz Quad' stands for in some site names.</rdfs:comment>
  </owl:Class>
  <owl:Class rdf:about="https://cn.dataone.org/cn/v2/object/doi:10.5063/F1B8562K#d_2_c_5">
    <rdfs:comment>Date of quadrat sampling where known. Four digit year is put where no date could be found, but may be able to corrobrate with 'dateVisits.csv' table. Unsure what 'not so good' stands for.</rdfs:comment>
    <rdfs:subClassOf rdf:resource="http://ecoinformatics.org/oboe/oboe.1.1/oboe-core.owl#Characteristic"/>
  </owl:Class>
  <owl:Class rdf:about="https://cn.dataone.org/cn/v2/object/doi:10.5063/F1B8562K#d_1_c_3">
    <rdfs:subClassOf rdf:resource="http://ecoinformatics.org/oboe/oboe.1.1/oboe-core.owl#Characteristic"/>
    <rdfs:comment>Sample site name, 11 sites total. Unsure what the 'Liz Quad' stands for in some site names.</rdfs:comment>
  </owl:Class>
  <owl:Class rdf:about="https://cn.dataone.org/cn/v2/object/doi:10.5063/F1B8562K#d_2_c_3">
    <rdfs:subClassOf rdf:resource="http://ecoinformatics.org/oboe/oboe.1.1/oboe-core.owl#Characteristic"/>
    <rdfs:comment>Date of quadrat sampling where known. Four digit year is put where no date could be found, but may be able to corrobrate with 'dateVisits.csv' table. Unsure what 'not so good' stands for.</rdfs:comment>
  </owl:Class>
  <owl:Class rdf:about="https://cn.dataone.org/cn/v2/object/doi:10.5063/F1B8562K#d_1_c_1">
    <rdfs:comment>Sample site name, 11 sites total. Unsure what the 'Liz Quad' stands for in some site names.</rdfs:comment>
    <rdfs:subClassOf rdf:resource="http://ecoinformatics.org/oboe/oboe.1.1/oboe-core.owl#Characteristic"/>
  </owl:Class>
</rdf:RDF>
