<?xml version="1.0" encoding="utf-8"?>
<rdf:RDF
  xmlns:owl="http://www.w3.org/2002/07/owl#"
  xmlns:rdf="http://www.w3.org/1999/02/22-rdf-syntax-ns#"
  xmlns:rdfs="http://www.w3.org/2000/01/rdf-schema#"
>
  <owl:Class rdf:about="https://cn.dataone.org/cn/v2/object/doi:10.5063/AA/bowdish.258.6#d_1_a_7">
    <rdfs:label>Summary Table of Marine Protected Areas </rdfs:label>
    <rdfs:subClassOf>
      <owl:Restriction rdf:nodeID="Nc8a4d61b396c4dc9a50e78721978b7ce">
        <owl:someValuesFrom rdf:resource="https://cn.dataone.org/cn/v2/object/doi:10.5063/AA/bowdish.258.6#d_1_c_7"/>
        <owl:onProperty rdf:resource="http://ecoinformatics.org/oboe/oboe.1.1/oboe-core.owl#measuresCharacteristic"/>
      </owl:Restriction>
    </rdfs:subClassOf>
    <rdfs:subClassOf>
      <owl:Restriction rdf:nodeID="N93f5305ed29f41d0aaf10e05be97f305">
        <owl:someValuesFrom rdf:resource="https://cn.dataone.org/cn/v2/object/doi:10.5063/AA/bowdish.258.6#d_1"/>
        <owl:onProperty rdf:resource="http://ecoinformatics.org/oboe/oboe.1.1/oboe-core.owl#measuresEntity"/>
      </owl:Restriction>
    </rdfs:subClassOf>
    <rdfs:subClassOf rdf:resource="http://ecoinformatics.org/oboe/oboe.1.1/oboe-core.owl#MeasurementType"/>
  </owl:Class>
  <owl:Class rdf:about="https://cn.dataone.org/cn/v2/object/doi:10.5063/AA/bowdish.258.6#d_1_a_4">
    <rdfs:subClassOf rdf:resource="http://ecoinformatics.org/oboe/oboe.1.1/oboe-core.owl#MeasurementType"/>
    <rdfs:label>Summary Table of Marine Protected Areas </rdfs:label>
    <rdfs:subClassOf>
      <owl:Restriction rdf:nodeID="N00a2be70ad8b478a8bee54c5997ff1d3">
        <owl:onProperty rdf:resource="http://ecoinformatics.org/oboe/oboe.1.1/oboe-core.owl#measuresCharacteristic"/>
        <owl:someValuesFrom rdf:resource="https://cn.dataone.org/cn/v2/object/doi:10.5063/AA/bowdish.258.6#d_1_c_4"/>
      </owl:Restriction>
    </rdfs:subClassOf>
    <rdfs:subClassOf>
      <owl:Restriction rdf:nodeID="Ndff965c4aa2b4d0eb9ddda37fae15cb7">
        <owl:someValuesFrom rdf:resource="https://cn.dataone.org/cn/v2/object/doi:10.5063/AA/bowdish.258.6#d_1"/>
        <owl:onProperty rdf:resource="http://ecoinformatics.org/oboe/oboe.1.1/oboe-core.owl#measuresEntity"/>
      </owl:Restriction>
    </rdfs:subClassOf>
  </owl:Class>
  <owl:Class rdf:about="https://cn.dataone.org/cn/v2/object/doi:10.5063/AA/bowdish.258.6#d_1_a_5">
    <rdfs:subClassOf>
      <owl:Restriction rdf:nodeID="N0cd043cd992147139d997ae9272d3414">
        <owl:someValuesFrom rdf:resource="https://cn.dataone.org/cn/v2/object/doi:10.5063/AA/bowdish.258.6#d_1_c_5"/>
        <owl:onProperty rdf:resource="http://ecoinformatics.org/oboe/oboe.1.1/oboe-core.owl#measuresCharacteristic"/>
      </owl:Restriction>
    </rdfs:subClassOf>
    <rdfs:subClassOf rdf:resource="http://ecoinformatics.org/oboe/oboe.1.1/oboe-core.owl#MeasurementType"/>
    <rdfs:label>Summary Table of Marine Protected Areas </rdfs:label>
    <rdfs:subClassOf>
      <owl:Restriction rdf:nodeID="Ne48e445be0a24eb0a1a083793b3dd74e">
        <owl:onProperty rdf:resource="http://ecoinformatics.org/oboe/oboe.1.1/oboe-core.owl#measuresEntity"/>
        <owl:someValuesFrom rdf:resource="https://cn.dataone.org/cn/v2/object/doi:10.5063/AA/bowdish.258.6#d_1"/>
      </owl:Restriction>
    </rdfs:subClassOf>
  </owl:Class>
  <owl:Ontology rdf:about="https://cn.dataone.org/cn/v2/object/doi:10.5063/AA/bowdish.258.6">
    <rdfs:label>Summary table of Marine Protected areas</rdfs:label>
    <rdfs:comment>This is a summary table of Marine Protected Areas (MPA) studies from which data on responses of species and functional diversity to protection were extracted. This table is refered to in a paper titled:  Micheli, Fiorenza&amp; Halpern, Benjamin S. (2005) Low functional redundancy in coastal marine assemblages. Ecology Letters 8 (4), 391-400. doi: 10.1111/ j.1461-0248.2005.00731.x</rdfs:comment>
  </owl:Ontology>
  <owl:Class rdf:about="https://cn.dataone.org/cn/v2/object/doi:10.5063/AA/bowdish.258.6#d_1_a_2">
    <rdfs:subClassOf rdf:resource="http://ecoinformatics.org/oboe/oboe.1.1/oboe-core.owl#MeasurementType"/>
    <rdfs:subClassOf>
      <owl:Restriction rdf:nodeID="Nc3f63eda0e5843a2b5a5f72776c63762">
        <owl:onProperty rdf:resource="http://ecoinformatics.org/oboe/oboe.1.1/oboe-core.owl#measuresCharacteristic"/>
        <owl:someValuesFrom rdf:resource="https://cn.dataone.org/cn/v2/object/doi:10.5063/AA/bowdish.258.6#d_1_c_2"/>
      </owl:Restriction>
    </rdfs:subClassOf>
    <rdfs:subClassOf>
      <owl:Restriction rdf:nodeID="N86b1d27f1a3246aa965329498c5757df">
        <owl:onProperty rdf:resource="http://ecoinformatics.org/oboe/oboe.1.1/oboe-core.owl#measuresEntity"/>
        <owl:someValuesFrom rdf:resource="https://cn.dataone.org/cn/v2/object/doi:10.5063/AA/bowdish.258.6#d_1"/>
      </owl:Restriction>
    </rdfs:subClassOf>
    <rdfs:label>Summary Table of Marine Protected Areas </rdfs:label>
  </owl:Class>
  <owl:Class rdf:about="https://cn.dataone.org/cn/v2/object/doi:10.5063/AA/bowdish.258.6#d_1_a_6">
    <rdfs:label>Summary Table of Marine Protected Areas </rdfs:label>
    <rdfs:subClassOf>
      <owl:Restriction rdf:nodeID="N04c448febf84434eb9218676eda9e4a0">
        <owl:someValuesFrom rdf:resource="https://cn.dataone.org/cn/v2/object/doi:10.5063/AA/bowdish.258.6#d_1"/>
        <owl:onProperty rdf:resource="http://ecoinformatics.org/oboe/oboe.1.1/oboe-core.owl#measuresEntity"/>
      </owl:Restriction>
    </rdfs:subClassOf>
    <rdfs:subClassOf rdf:resource="http://ecoinformatics.org/oboe/oboe.1.1/oboe-core.owl#MeasurementType"/>
    <rdfs:subClassOf>
      <owl:Restriction rdf:nodeID="Nfc75aeeb23584457bc741be7082c6b2a">
        <owl:someValuesFrom rdf:resource="https://cn.dataone.org/cn/v2/object/doi:10.5063/AA/bowdish.258.6#d_1_c_6"/>
        <owl:onProperty rdf:resource="http://ecoinformatics.org/oboe/oboe.1.1/oboe-core.owl#measuresCharacteristic"/>
      </owl:Restriction>
    </rdfs:subClassOf>
  </owl:Class>
  <owl:Class rdf:about="https://cn.dataone.org/cn/v2/object/doi:10.5063/AA/bowdish.258.6#d_1_a_1">
    <rdfs:subClassOf rdf:resource="http://ecoinformatics.org/oboe/oboe.1.1/oboe-core.owl#MeasurementType"/>
    <rdfs:subClassOf>
      <owl:Restriction rdf:nodeID="N7d6b2902a923460ca4d6efd54a54bc9f">
        <owl:someValuesFrom rdf:resource="https://cn.dataone.org/cn/v2/object/doi:10.5063/AA/bowdish.258.6#d_1"/>
        <owl:onProperty rdf:resource="http://ecoinformatics.org/oboe/oboe.1.1/oboe-core.owl#measuresEntity"/>
      </owl:Restriction>
    </rdfs:subClassOf>
    <rdfs:label>Summary Table of Marine Protected Areas </rdfs:label>
    <rdfs:subClassOf>
      <owl:Restriction rdf:nodeID="N0a804343aa684686ae2334ee2f851aa8">
        <owl:someValuesFrom rdf:resource="https://cn.dataone.org/cn/v2/object/doi:10.5063/AA/bowdish.258.6#d_1_c_1"/>
        <owl:onProperty rdf:resource="http://ecoinformatics.org/oboe/oboe.1.1/oboe-core.owl#measuresCharacteristic"/>
      </owl:Restriction>
    </rdfs:subClassOf>
  </owl:Class>
  <owl:Class rdf:about="https://cn.dataone.org/cn/v2/object/doi:10.5063/AA/bowdish.258.6#d_1_a_3">
    <rdfs:subClassOf rdf:resource="http://ecoinformatics.org/oboe/oboe.1.1/oboe-core.owl#MeasurementType"/>
    <rdfs:label>Summary Table of Marine Protected Areas </rdfs:label>
    <rdfs:subClassOf>
      <owl:Restriction rdf:nodeID="N9779cbd3f5354bd3867664404b9fa0aa">
        <owl:onProperty rdf:resource="http://ecoinformatics.org/oboe/oboe.1.1/oboe-core.owl#measuresCharacteristic"/>
        <owl:someValuesFrom rdf:resource="https://cn.dataone.org/cn/v2/object/doi:10.5063/AA/bowdish.258.6#d_1_c_3"/>
      </owl:Restriction>
    </rdfs:subClassOf>
    <rdfs:subClassOf>
      <owl:Restriction rdf:nodeID="N50ec665dfc4e424eb1498ef99981eb82">
        <owl:onProperty rdf:resource="http://ecoinformatics.org/oboe/oboe.1.1/oboe-core.owl#measuresEntity"/>
        <owl:someValuesFrom rdf:resource="https://cn.dataone.org/cn/v2/object/doi:10.5063/AA/bowdish.258.6#d_1"/>
      </owl:Restriction>
    </rdfs:subClassOf>
  </owl:Class>
  <owl:Class rdf:about="https://cn.dataone.org/cn/v2/object/doi:10.5063/AA/bowdish.258.6#d_1">
    <rdfs:subClassOf rdf:resource="http://ecoinformatics.org/oboe/oboe.1.1/oboe-core.owl#Entity"/>
    <rdfs:comment>Summary table of MPA studies from which data on responses of species and functional diversity to protection were extracted.</rdfs:comment>
    <rdfs:label>Summary Table of Marine Protected Areas</rdfs:label>
  </owl:Class>
  <owl:Class rdf:about="https://cn.dataone.org/cn/v2/object/doi:10.5063/AA/bowdish.258.6#d_1_c_1">
    <rdfs:comment>This is the location of Marine Protected Areas, The number is the reference that was used. The references are listed in the additional information area of this data set.</rdfs:comment>
    <rdfs:subClassOf rdf:resource="http://ecoinformatics.org/oboe/oboe.1.1/oboe-core.owl#Characteristic"/>
  </owl:Class>
  <owl:Class rdf:about="https://cn.dataone.org/cn/v2/object/doi:10.5063/AA/bowdish.258.6#d_1_c_6">
    <rdfs:comment>This is the location of Marine Protected Areas, The number is the reference that was used. The references are listed in the additional information area of this data set.</rdfs:comment>
    <rdfs:subClassOf rdf:resource="http://ecoinformatics.org/oboe/oboe.1.1/oboe-core.owl#Characteristic"/>
  </owl:Class>
  <owl:Class rdf:about="https://cn.dataone.org/cn/v2/object/doi:10.5063/AA/bowdish.258.6#d_1_c_5">
    <rdfs:subClassOf rdf:resource="http://ecoinformatics.org/oboe/oboe.1.1/oboe-core.owl#Characteristic"/>
    <rdfs:comment>This is the location of Marine Protected Areas, The number is the reference that was used. The references are listed in the additional information area of this data set.</rdfs:comment>
  </owl:Class>
  <owl:Class rdf:about="https://cn.dataone.org/cn/v2/object/doi:10.5063/AA/bowdish.258.6#d_1_c_3">
    <rdfs:comment>This is the location of Marine Protected Areas, The number is the reference that was used. The references are listed in the additional information area of this data set.</rdfs:comment>
    <rdfs:subClassOf rdf:resource="http://ecoinformatics.org/oboe/oboe.1.1/oboe-core.owl#Characteristic"/>
  </owl:Class>
  <owl:Class rdf:about="https://cn.dataone.org/cn/v2/object/doi:10.5063/AA/bowdish.258.6#d_1_c_7">
    <rdfs:comment>This is the location of Marine Protected Areas, The number is the reference that was used. The references are listed in the additional information area of this data set.</rdfs:comment>
    <rdfs:subClassOf rdf:resource="http://ecoinformatics.org/oboe/oboe.1.1/oboe-core.owl#Characteristic"/>
  </owl:Class>
  <owl:Class rdf:about="https://cn.dataone.org/cn/v2/object/doi:10.5063/AA/bowdish.258.6#d_1_c_4">
    <rdfs:subClassOf rdf:resource="http://ecoinformatics.org/oboe/oboe.1.1/oboe-core.owl#Characteristic"/>
    <rdfs:comment>This is the location of Marine Protected Areas, The number is the reference that was used. The references are listed in the additional information area of this data set.</rdfs:comment>
  </owl:Class>
  <owl:Class rdf:about="https://cn.dataone.org/cn/v2/object/doi:10.5063/AA/bowdish.258.6#d_1_c_2">
    <rdfs:subClassOf rdf:resource="http://ecoinformatics.org/oboe/oboe.1.1/oboe-core.owl#Characteristic"/>
    <rdfs:comment>This is the location of Marine Protected Areas, The number is the reference that was used. The references are listed in the additional information area of this data set.</rdfs:comment>
  </owl:Class>
</rdf:RDF>
