<?xml version="1.0" encoding="utf-8"?>
<rdf:RDF
  xmlns:owl="http://www.w3.org/2002/07/owl#"
  xmlns:rdf="http://www.w3.org/1999/02/22-rdf-syntax-ns#"
  xmlns:rdfs="http://www.w3.org/2000/01/rdf-schema#"
>
  <owl:Class rdf:about="https://cn.dataone.org/cn/v2/object/https://pasta.lternet.edu/package/metadata/eml/knb-lter-sbc/3001/6#d_1_a_1">
    <rdfs:subClassOf>
      <owl:Restriction rdf:nodeID="N417b6aacf3484981948521fc61b3d00a">
        <owl:onProperty rdf:resource="http://ecoinformatics.org/oboe/oboe.1.1/oboe-core.owl#measuresEntity"/>
        <owl:someValuesFrom rdf:resource="https://cn.dataone.org/cn/v2/object/https://pasta.lternet.edu/package/metadata/eml/knb-lter-sbc/3001/6#d_1"/>
      </owl:Restriction>
    </rdfs:subClassOf>
    <rdfs:label>Discharge SBC AB00, all years Date and Time, local</rdfs:label>
    <rdfs:subClassOf rdf:resource="http://ecoinformatics.org/oboe/oboe.1.1/oboe-core.owl#MeasurementType"/>
    <rdfs:subClassOf>
      <owl:Restriction rdf:nodeID="N0922e1316db94bd592241f8d9823676b">
        <owl:someValuesFrom rdf:resource="https://cn.dataone.org/cn/v2/object/https://pasta.lternet.edu/package/metadata/eml/knb-lter-sbc/3001/6#d_1_c_1"/>
        <owl:onProperty rdf:resource="http://ecoinformatics.org/oboe/oboe.1.1/oboe-core.owl#measuresCharacteristic"/>
      </owl:Restriction>
    </rdfs:subClassOf>
  </owl:Class>
  <owl:Class rdf:about="https://cn.dataone.org/cn/v2/object/https://pasta.lternet.edu/package/metadata/eml/knb-lter-sbc/3001/6#d_1_a_2">
    <rdfs:subClassOf rdf:resource="http://ecoinformatics.org/oboe/oboe.1.1/oboe-core.owl#MeasurementType"/>
    <rdfs:subClassOf>
      <owl:Restriction rdf:nodeID="N21fb2991343d418a9abc4a855cfb9f9d">
        <owl:someValuesFrom rdf:resource="https://cn.dataone.org/cn/v2/object/https://pasta.lternet.edu/package/metadata/eml/knb-lter-sbc/3001/6#d_1"/>
        <owl:onProperty rdf:resource="http://ecoinformatics.org/oboe/oboe.1.1/oboe-core.owl#measuresEntity"/>
      </owl:Restriction>
    </rdfs:subClassOf>
    <rdfs:subClassOf>
      <owl:Restriction rdf:nodeID="N9dd5bb44e1674fb599697aa4972a8f36">
        <owl:someValuesFrom rdf:resource="https://cn.dataone.org/cn/v2/object/https://pasta.lternet.edu/package/metadata/eml/knb-lter-sbc/3001/6#d_1_c_2"/>
        <owl:onProperty rdf:resource="http://ecoinformatics.org/oboe/oboe.1.1/oboe-core.owl#measuresCharacteristic"/>
      </owl:Restriction>
    </rdfs:subClassOf>
    <rdfs:label>Discharge SBC AB00, all years Date and Time, local</rdfs:label>
  </owl:Class>
  <owl:Class rdf:about="https://cn.dataone.org/cn/v2/object/https://pasta.lternet.edu/package/metadata/eml/knb-lter-sbc/3001/6#d_1_a_3">
    <rdfs:subClassOf rdf:resource="http://ecoinformatics.org/oboe/oboe.1.1/oboe-core.owl#MeasurementType"/>
    <rdfs:subClassOf>
      <owl:Restriction rdf:nodeID="Nb6cde4bc1db548a69a70753e85b46072">
        <owl:someValuesFrom rdf:resource="https://cn.dataone.org/cn/v2/object/https://pasta.lternet.edu/package/metadata/eml/knb-lter-sbc/3001/6#d_1"/>
        <owl:onProperty rdf:resource="http://ecoinformatics.org/oboe/oboe.1.1/oboe-core.owl#measuresEntity"/>
      </owl:Restriction>
    </rdfs:subClassOf>
    <rdfs:label>Discharge SBC AB00, all years Date and Time, local</rdfs:label>
    <rdfs:subClassOf>
      <owl:Restriction rdf:nodeID="Nde49a5721ee04c2cbd695ab52ee5bce0">
        <owl:onProperty rdf:resource="http://ecoinformatics.org/oboe/oboe.1.1/oboe-core.owl#measuresCharacteristic"/>
        <owl:someValuesFrom rdf:resource="https://cn.dataone.org/cn/v2/object/https://pasta.lternet.edu/package/metadata/eml/knb-lter-sbc/3001/6#d_1_c_3"/>
      </owl:Restriction>
    </rdfs:subClassOf>
  </owl:Class>
  <owl:Class rdf:about="https://cn.dataone.org/cn/v2/object/https://pasta.lternet.edu/package/metadata/eml/knb-lter-sbc/3001/6#d_1_a_4">
    <rdfs:subClassOf rdf:resource="http://ecoinformatics.org/oboe/oboe.1.1/oboe-core.owl#MeasurementType"/>
    <rdfs:subClassOf>
      <owl:Restriction rdf:nodeID="Nda5ee945aa1e49c2a66052bcd3dc89e2">
        <owl:onProperty rdf:resource="http://ecoinformatics.org/oboe/oboe.1.1/oboe-core.owl#measuresCharacteristic"/>
        <owl:someValuesFrom rdf:resource="https://cn.dataone.org/cn/v2/object/https://pasta.lternet.edu/package/metadata/eml/knb-lter-sbc/3001/6#d_1_c_4"/>
      </owl:Restriction>
    </rdfs:subClassOf>
    <rdfs:label>Discharge SBC AB00, all years Date and Time, local</rdfs:label>
    <rdfs:subClassOf>
      <owl:Restriction rdf:nodeID="N30ec2392b2b74af6be1ce94f59150a54">
        <owl:someValuesFrom rdf:resource="https://cn.dataone.org/cn/v2/object/https://pasta.lternet.edu/package/metadata/eml/knb-lter-sbc/3001/6#d_1"/>
        <owl:onProperty rdf:resource="http://ecoinformatics.org/oboe/oboe.1.1/oboe-core.owl#measuresEntity"/>
      </owl:Restriction>
    </rdfs:subClassOf>
  </owl:Class>
  <owl:Ontology rdf:about="https://cn.dataone.org/cn/v2/object/https://pasta.lternet.edu/package/metadata/eml/knb-lter-sbc/3001/6">
    <rdfs:label>SBC LTER: Land: Hydrology: Stream discharge and associated parameters at Arroyo Burro Creek, Cliff Drive (AB00)</rdfs:label>
    <rdfs:comment>Stream Discharge and water temperature were collected with a Solinst Model 3001 LT Levelogger at Arroyo Burro Creek, Cliff Drive in the Santa Barbara coastal area (site ID: AB00). Data are reported hourly. Stage values were converted to discharge using a rating curve developed with stream channel cross-sections, roughness estimates and the HEC-RAS model.</rdfs:comment>
  </owl:Ontology>
  <owl:Class rdf:about="https://cn.dataone.org/cn/v2/object/https://pasta.lternet.edu/package/metadata/eml/knb-lter-sbc/3001/6#d_1_c_2">
    <rdfs:comment>local time of observation, PST (-08:00 from UTC) or PDT (-07:00 from UTC)</rdfs:comment>
    <rdfs:label>Date and Time, local</rdfs:label>
    <rdfs:subClassOf rdf:resource="http://ecoinformatics.org/oboe/oboe.1.1/oboe-core.owl#Characteristic"/>
  </owl:Class>
  <owl:Class rdf:about="https://cn.dataone.org/cn/v2/object/https://pasta.lternet.edu/package/metadata/eml/knb-lter-sbc/3001/6#d_1">
    <rdfs:label>Discharge SBC AB00, all years</rdfs:label>
    <rdfs:comment>Stream discharge data from Arroyo Burro Creek, Cliff Drive (station = AB00) including water temperature (2001-11-19 - 2011-09-29)</rdfs:comment>
    <rdfs:subClassOf rdf:resource="http://ecoinformatics.org/oboe/oboe.1.1/oboe-core.owl#Entity"/>
  </owl:Class>
  <owl:Class rdf:about="https://cn.dataone.org/cn/v2/object/https://pasta.lternet.edu/package/metadata/eml/knb-lter-sbc/3001/6#d_1_c_3">
    <rdfs:label>Date and Time, local</rdfs:label>
    <rdfs:subClassOf rdf:resource="http://ecoinformatics.org/oboe/oboe.1.1/oboe-core.owl#Characteristic"/>
    <rdfs:comment>local time of observation, PST (-08:00 from UTC) or PDT (-07:00 from UTC)</rdfs:comment>
  </owl:Class>
  <owl:Class rdf:about="https://cn.dataone.org/cn/v2/object/https://pasta.lternet.edu/package/metadata/eml/knb-lter-sbc/3001/6#d_1_c_1">
    <rdfs:comment>local time of observation, PST (-08:00 from UTC) or PDT (-07:00 from UTC)</rdfs:comment>
    <rdfs:subClassOf rdf:resource="http://ecoinformatics.org/oboe/oboe.1.1/oboe-core.owl#Characteristic"/>
    <rdfs:label>Date and Time, local</rdfs:label>
  </owl:Class>
  <owl:Class rdf:about="https://cn.dataone.org/cn/v2/object/https://pasta.lternet.edu/package/metadata/eml/knb-lter-sbc/3001/6#d_1_c_4">
    <rdfs:comment>local time of observation, PST (-08:00 from UTC) or PDT (-07:00 from UTC)</rdfs:comment>
    <rdfs:label>Date and Time, local</rdfs:label>
    <rdfs:subClassOf rdf:resource="http://ecoinformatics.org/oboe/oboe.1.1/oboe-core.owl#Characteristic"/>
  </owl:Class>
</rdf:RDF>
