<?xml version="1.0" encoding="utf-8"?>
<rdf:RDF
  xmlns:owl="http://www.w3.org/2002/07/owl#"
  xmlns:rdf="http://www.w3.org/1999/02/22-rdf-syntax-ns#"
  xmlns:rdfs="http://www.w3.org/2000/01/rdf-schema#"
>
  <owl:Class rdf:about="https://cn.dataone.org/cn/v2/object/https://pasta.lternet.edu/package/metadata/eml/knb-lter-sbc/5007/5#d_1_a_1">
    <rdfs:subClassOf rdf:resource="http://ecoinformatics.org/oboe/oboe.1.1/oboe-core.owl#MeasurementType"/>
    <rdfs:subClassOf>
      <owl:Restriction rdf:nodeID="N7a98798ded2b414f9232f2a0237a4e2e">
        <owl:someValuesFrom rdf:resource="https://cn.dataone.org/cn/v2/object/https://pasta.lternet.edu/package/metadata/eml/knb-lter-sbc/5007/5#d_1_c_1"/>
        <owl:onProperty rdf:resource="http://ecoinformatics.org/oboe/oboe.1.1/oboe-core.owl#measuresCharacteristic"/>
      </owl:Restriction>
    </rdfs:subClassOf>
    <rdfs:subClassOf>
      <owl:Restriction rdf:nodeID="N03716d9aa6e6426fb5045111cbc33a66">
        <owl:someValuesFrom rdf:resource="https://cn.dataone.org/cn/v2/object/https://pasta.lternet.edu/package/metadata/eml/knb-lter-sbc/5007/5#d_1"/>
        <owl:onProperty rdf:resource="http://ecoinformatics.org/oboe/oboe.1.1/oboe-core.owl#measuresEntity"/>
      </owl:Restriction>
    </rdfs:subClassOf>
    <rdfs:label>Precipitation SBCoFC Edison Trail 252, all years Date and Time, local</rdfs:label>
  </owl:Class>
  <owl:Ontology rdf:about="https://cn.dataone.org/cn/v2/object/https://pasta.lternet.edu/package/metadata/eml/knb-lter-sbc/5007/5">
    <rdfs:comment>Precipitation was collected by the Santa Barbara County Flood Control District at Edison Trail in the Santa Barbara coastal area (site ID: EdisonTrail252). Data are reported at 5 minute intervals. For more information, see http://www.countyofsb.org/pwd/.</rdfs:comment>
    <rdfs:label>SBC LTER: Land: Hydrology: Santa Barbara County Flood Control District - Precipitation at Edison Trail (EdisonTrail252)</rdfs:label>
  </owl:Ontology>
  <owl:Class rdf:about="https://cn.dataone.org/cn/v2/object/https://pasta.lternet.edu/package/metadata/eml/knb-lter-sbc/5007/5#d_1_a_3">
    <rdfs:subClassOf>
      <owl:Restriction rdf:nodeID="N1234ecbb1698499081df60e365854da4">
        <owl:onProperty rdf:resource="http://ecoinformatics.org/oboe/oboe.1.1/oboe-core.owl#measuresEntity"/>
        <owl:someValuesFrom rdf:resource="https://cn.dataone.org/cn/v2/object/https://pasta.lternet.edu/package/metadata/eml/knb-lter-sbc/5007/5#d_1"/>
      </owl:Restriction>
    </rdfs:subClassOf>
    <rdfs:label>Precipitation SBCoFC Edison Trail 252, all years Date and Time, local</rdfs:label>
    <rdfs:subClassOf>
      <owl:Restriction rdf:nodeID="N6db6a267825b41a4857b5d05a673765a">
        <owl:onProperty rdf:resource="http://ecoinformatics.org/oboe/oboe.1.1/oboe-core.owl#measuresCharacteristic"/>
        <owl:someValuesFrom rdf:resource="https://cn.dataone.org/cn/v2/object/https://pasta.lternet.edu/package/metadata/eml/knb-lter-sbc/5007/5#d_1_c_3"/>
      </owl:Restriction>
    </rdfs:subClassOf>
    <rdfs:subClassOf rdf:resource="http://ecoinformatics.org/oboe/oboe.1.1/oboe-core.owl#MeasurementType"/>
  </owl:Class>
  <owl:Class rdf:about="https://cn.dataone.org/cn/v2/object/https://pasta.lternet.edu/package/metadata/eml/knb-lter-sbc/5007/5#d_1_a_2">
    <rdfs:subClassOf rdf:resource="http://ecoinformatics.org/oboe/oboe.1.1/oboe-core.owl#MeasurementType"/>
    <rdfs:label>Precipitation SBCoFC Edison Trail 252, all years Date and Time, local</rdfs:label>
    <rdfs:subClassOf>
      <owl:Restriction rdf:nodeID="N339dd876e91448be94403d959b5966ed">
        <owl:onProperty rdf:resource="http://ecoinformatics.org/oboe/oboe.1.1/oboe-core.owl#measuresCharacteristic"/>
        <owl:someValuesFrom rdf:resource="https://cn.dataone.org/cn/v2/object/https://pasta.lternet.edu/package/metadata/eml/knb-lter-sbc/5007/5#d_1_c_2"/>
      </owl:Restriction>
    </rdfs:subClassOf>
    <rdfs:subClassOf>
      <owl:Restriction rdf:nodeID="Nf1cecba87cda4370af3ce4085c6aea43">
        <owl:onProperty rdf:resource="http://ecoinformatics.org/oboe/oboe.1.1/oboe-core.owl#measuresEntity"/>
        <owl:someValuesFrom rdf:resource="https://cn.dataone.org/cn/v2/object/https://pasta.lternet.edu/package/metadata/eml/knb-lter-sbc/5007/5#d_1"/>
      </owl:Restriction>
    </rdfs:subClassOf>
  </owl:Class>
  <owl:Class rdf:about="https://cn.dataone.org/cn/v2/object/https://pasta.lternet.edu/package/metadata/eml/knb-lter-sbc/5007/5#d_1_c_3">
    <rdfs:subClassOf rdf:resource="http://ecoinformatics.org/oboe/oboe.1.1/oboe-core.owl#Characteristic"/>
    <rdfs:comment>local time of observation, no correction for daylight saving time</rdfs:comment>
    <rdfs:label>Date and Time, local</rdfs:label>
  </owl:Class>
  <owl:Class rdf:about="https://cn.dataone.org/cn/v2/object/https://pasta.lternet.edu/package/metadata/eml/knb-lter-sbc/5007/5#d_1">
    <rdfs:subClassOf rdf:resource="http://ecoinformatics.org/oboe/oboe.1.1/oboe-core.owl#Entity"/>
    <rdfs:label>Precipitation SBCoFC Edison Trail 252, all years</rdfs:label>
    <rdfs:comment>SBCo PWD Precipitation data from Edison Trail (station = EdisonTrail252) from 2000-10-01 to 2008-09-30.</rdfs:comment>
  </owl:Class>
  <owl:Class rdf:about="https://cn.dataone.org/cn/v2/object/https://pasta.lternet.edu/package/metadata/eml/knb-lter-sbc/5007/5#d_1_c_2">
    <rdfs:label>Date and Time, local</rdfs:label>
    <rdfs:comment>local time of observation, no correction for daylight saving time</rdfs:comment>
    <rdfs:subClassOf rdf:resource="http://ecoinformatics.org/oboe/oboe.1.1/oboe-core.owl#Characteristic"/>
  </owl:Class>
  <owl:Class rdf:about="https://cn.dataone.org/cn/v2/object/https://pasta.lternet.edu/package/metadata/eml/knb-lter-sbc/5007/5#d_1_c_1">
    <rdfs:subClassOf rdf:resource="http://ecoinformatics.org/oboe/oboe.1.1/oboe-core.owl#Characteristic"/>
    <rdfs:comment>local time of observation, no correction for daylight saving time</rdfs:comment>
    <rdfs:label>Date and Time, local</rdfs:label>
  </owl:Class>
</rdf:RDF>
