<?xml version="1.0" encoding="utf-8"?>
<rdf:RDF
  xmlns:owl="http://www.w3.org/2002/07/owl#"
  xmlns:rdf="http://www.w3.org/1999/02/22-rdf-syntax-ns#"
  xmlns:rdfs="http://www.w3.org/2000/01/rdf-schema#"
>
  <owl:Class rdf:about="https://cn.dataone.org/cn/v2/object/https://pasta.lternet.edu/package/metadata/eml/knb-lter-sbc/4006/7#d_1_a_3">
    <rdfs:subClassOf rdf:resource="http://ecoinformatics.org/oboe/oboe.1.1/oboe-core.owl#MeasurementType"/>
    <rdfs:label>Precipitation SBC GV202, all years Date and Time, local</rdfs:label>
    <rdfs:subClassOf>
      <owl:Restriction rdf:nodeID="Na9069961dab143c4809daa0bfccd1b93">
        <owl:onProperty rdf:resource="http://ecoinformatics.org/oboe/oboe.1.1/oboe-core.owl#measuresEntity"/>
        <owl:someValuesFrom rdf:resource="https://cn.dataone.org/cn/v2/object/https://pasta.lternet.edu/package/metadata/eml/knb-lter-sbc/4006/7#d_1"/>
      </owl:Restriction>
    </rdfs:subClassOf>
    <rdfs:subClassOf>
      <owl:Restriction rdf:nodeID="N67d089d20a8c489e9fc519eb8a7e4453">
        <owl:someValuesFrom rdf:resource="https://cn.dataone.org/cn/v2/object/https://pasta.lternet.edu/package/metadata/eml/knb-lter-sbc/4006/7#d_1_c_3"/>
        <owl:onProperty rdf:resource="http://ecoinformatics.org/oboe/oboe.1.1/oboe-core.owl#measuresCharacteristic"/>
      </owl:Restriction>
    </rdfs:subClassOf>
  </owl:Class>
  <owl:Class rdf:about="https://cn.dataone.org/cn/v2/object/https://pasta.lternet.edu/package/metadata/eml/knb-lter-sbc/4006/7#d_1_a_1">
    <rdfs:subClassOf>
      <owl:Restriction rdf:nodeID="N82ea70ec7d4c428a8ac0279733a29450">
        <owl:someValuesFrom rdf:resource="https://cn.dataone.org/cn/v2/object/https://pasta.lternet.edu/package/metadata/eml/knb-lter-sbc/4006/7#d_1"/>
        <owl:onProperty rdf:resource="http://ecoinformatics.org/oboe/oboe.1.1/oboe-core.owl#measuresEntity"/>
      </owl:Restriction>
    </rdfs:subClassOf>
    <rdfs:label>Precipitation SBC GV202, all years Date and Time, local</rdfs:label>
    <rdfs:subClassOf rdf:resource="http://ecoinformatics.org/oboe/oboe.1.1/oboe-core.owl#MeasurementType"/>
    <rdfs:subClassOf>
      <owl:Restriction rdf:nodeID="N4bf9355a38f1444c8a8f055a54f257d2">
        <owl:someValuesFrom rdf:resource="https://cn.dataone.org/cn/v2/object/https://pasta.lternet.edu/package/metadata/eml/knb-lter-sbc/4006/7#d_1_c_1"/>
        <owl:onProperty rdf:resource="http://ecoinformatics.org/oboe/oboe.1.1/oboe-core.owl#measuresCharacteristic"/>
      </owl:Restriction>
    </rdfs:subClassOf>
  </owl:Class>
  <owl:Class rdf:about="https://cn.dataone.org/cn/v2/object/https://pasta.lternet.edu/package/metadata/eml/knb-lter-sbc/4006/7#d_1_a_2">
    <rdfs:subClassOf>
      <owl:Restriction rdf:nodeID="N6fb4b0bd897f42a4abbc39af6c1b26b9">
        <owl:someValuesFrom rdf:resource="https://cn.dataone.org/cn/v2/object/https://pasta.lternet.edu/package/metadata/eml/knb-lter-sbc/4006/7#d_1"/>
        <owl:onProperty rdf:resource="http://ecoinformatics.org/oboe/oboe.1.1/oboe-core.owl#measuresEntity"/>
      </owl:Restriction>
    </rdfs:subClassOf>
    <rdfs:subClassOf>
      <owl:Restriction rdf:nodeID="N08ad256692534505a7a87aa41f4788c1">
        <owl:onProperty rdf:resource="http://ecoinformatics.org/oboe/oboe.1.1/oboe-core.owl#measuresCharacteristic"/>
        <owl:someValuesFrom rdf:resource="https://cn.dataone.org/cn/v2/object/https://pasta.lternet.edu/package/metadata/eml/knb-lter-sbc/4006/7#d_1_c_2"/>
      </owl:Restriction>
    </rdfs:subClassOf>
    <rdfs:subClassOf rdf:resource="http://ecoinformatics.org/oboe/oboe.1.1/oboe-core.owl#MeasurementType"/>
    <rdfs:label>Precipitation SBC GV202, all years Date and Time, local</rdfs:label>
  </owl:Class>
  <owl:Ontology rdf:about="https://cn.dataone.org/cn/v2/object/https://pasta.lternet.edu/package/metadata/eml/knb-lter-sbc/4006/7">
    <rdfs:comment>Precipitation was collected at Gaviota at Las Cruces School in the Santa Barbara coastal area (site ID: GV202). A Tipping Bucket rain gauge from either Qualimetrics (Model 6011B) or Sutron (Model 5600-0425-2) was used.</rdfs:comment>
    <rdfs:label>SBC LTER: Land: Hydrology: Precipitation at Gaviota at Las Cruces School (GV202)</rdfs:label>
  </owl:Ontology>
  <owl:Class rdf:about="https://cn.dataone.org/cn/v2/object/https://pasta.lternet.edu/package/metadata/eml/knb-lter-sbc/4006/7#d_1_c_1">
    <rdfs:subClassOf rdf:resource="http://ecoinformatics.org/oboe/oboe.1.1/oboe-core.owl#Characteristic"/>
    <rdfs:comment>local time of observation, no correction for daylight saving time</rdfs:comment>
    <rdfs:label>Date and Time, local</rdfs:label>
  </owl:Class>
  <owl:Class rdf:about="https://cn.dataone.org/cn/v2/object/https://pasta.lternet.edu/package/metadata/eml/knb-lter-sbc/4006/7#d_1">
    <rdfs:subClassOf rdf:resource="http://ecoinformatics.org/oboe/oboe.1.1/oboe-core.owl#Entity"/>
    <rdfs:comment>Precipitation data from Gaviota at Las Cruces School (station = GV202) from 2002-10-01 to 2010-09-30.</rdfs:comment>
    <rdfs:label>Precipitation SBC GV202, all years</rdfs:label>
  </owl:Class>
  <owl:Class rdf:about="https://cn.dataone.org/cn/v2/object/https://pasta.lternet.edu/package/metadata/eml/knb-lter-sbc/4006/7#d_1_c_3">
    <rdfs:comment>local time of observation, no correction for daylight saving time</rdfs:comment>
    <rdfs:subClassOf rdf:resource="http://ecoinformatics.org/oboe/oboe.1.1/oboe-core.owl#Characteristic"/>
    <rdfs:label>Date and Time, local</rdfs:label>
  </owl:Class>
  <owl:Class rdf:about="https://cn.dataone.org/cn/v2/object/https://pasta.lternet.edu/package/metadata/eml/knb-lter-sbc/4006/7#d_1_c_2">
    <rdfs:label>Date and Time, local</rdfs:label>
    <rdfs:subClassOf rdf:resource="http://ecoinformatics.org/oboe/oboe.1.1/oboe-core.owl#Characteristic"/>
    <rdfs:comment>local time of observation, no correction for daylight saving time</rdfs:comment>
  </owl:Class>
</rdf:RDF>
