<?xml version="1.0" encoding="utf-8"?>
<rdf:RDF
  xmlns:owl="http://www.w3.org/2002/07/owl#"
  xmlns:rdf="http://www.w3.org/1999/02/22-rdf-syntax-ns#"
  xmlns:rdfs="http://www.w3.org/2000/01/rdf-schema#"
>
  <owl:Ontology rdf:about="https://cn.dataone.org/cn/v2/object/https://pasta.lternet.edu/package/metadata/eml/knb-lter-sbc/4004/6">
    <rdfs:label>SBC LTER: Land: Hydrology: Precipitation at Gobernador at Veddar's Ranch (GB201)</rdfs:label>
    <rdfs:comment>Precipitation was collected at Gobernador at Veddar's Ranch in the Santa Barbara coastal area (site ID: GB201).A Tipping Bucket rain gauge from either Qualimetrics (Model 6011B) or Sutron (Model 5600-0425-2) was used.</rdfs:comment>
  </owl:Ontology>
  <owl:Class rdf:about="https://cn.dataone.org/cn/v2/object/https://pasta.lternet.edu/package/metadata/eml/knb-lter-sbc/4004/6#d_1_a_3">
    <rdfs:label>Precipitation SBC GB201, all years Date and Time, local</rdfs:label>
    <rdfs:subClassOf>
      <owl:Restriction rdf:nodeID="N671c69b6c34642d59881727bb7e241f7">
        <owl:onProperty rdf:resource="http://ecoinformatics.org/oboe/oboe.1.1/oboe-core.owl#measuresEntity"/>
        <owl:someValuesFrom rdf:resource="https://cn.dataone.org/cn/v2/object/https://pasta.lternet.edu/package/metadata/eml/knb-lter-sbc/4004/6#d_1"/>
      </owl:Restriction>
    </rdfs:subClassOf>
    <rdfs:subClassOf>
      <owl:Restriction rdf:nodeID="N699e6e31755740ab854f441d2c3979e6">
        <owl:onProperty rdf:resource="http://ecoinformatics.org/oboe/oboe.1.1/oboe-core.owl#measuresCharacteristic"/>
        <owl:someValuesFrom rdf:resource="https://cn.dataone.org/cn/v2/object/https://pasta.lternet.edu/package/metadata/eml/knb-lter-sbc/4004/6#d_1_c_3"/>
      </owl:Restriction>
    </rdfs:subClassOf>
    <rdfs:subClassOf rdf:resource="http://ecoinformatics.org/oboe/oboe.1.1/oboe-core.owl#MeasurementType"/>
  </owl:Class>
  <owl:Class rdf:about="https://cn.dataone.org/cn/v2/object/https://pasta.lternet.edu/package/metadata/eml/knb-lter-sbc/4004/6#d_1_a_2">
    <rdfs:subClassOf>
      <owl:Restriction rdf:nodeID="Nf8644da6b6db47cca1d9e4df2299f6a9">
        <owl:someValuesFrom rdf:resource="https://cn.dataone.org/cn/v2/object/https://pasta.lternet.edu/package/metadata/eml/knb-lter-sbc/4004/6#d_1"/>
        <owl:onProperty rdf:resource="http://ecoinformatics.org/oboe/oboe.1.1/oboe-core.owl#measuresEntity"/>
      </owl:Restriction>
    </rdfs:subClassOf>
    <rdfs:subClassOf rdf:resource="http://ecoinformatics.org/oboe/oboe.1.1/oboe-core.owl#MeasurementType"/>
    <rdfs:subClassOf>
      <owl:Restriction rdf:nodeID="Ndb0906c181a74b308aab78ffe330cba6">
        <owl:onProperty rdf:resource="http://ecoinformatics.org/oboe/oboe.1.1/oboe-core.owl#measuresCharacteristic"/>
        <owl:someValuesFrom rdf:resource="https://cn.dataone.org/cn/v2/object/https://pasta.lternet.edu/package/metadata/eml/knb-lter-sbc/4004/6#d_1_c_2"/>
      </owl:Restriction>
    </rdfs:subClassOf>
    <rdfs:label>Precipitation SBC GB201, all years Date and Time, local</rdfs:label>
  </owl:Class>
  <owl:Class rdf:about="https://cn.dataone.org/cn/v2/object/https://pasta.lternet.edu/package/metadata/eml/knb-lter-sbc/4004/6#d_1_a_1">
    <rdfs:subClassOf>
      <owl:Restriction rdf:nodeID="Nf7fd6d1295cc480ea289a4890d58e001">
        <owl:someValuesFrom rdf:resource="https://cn.dataone.org/cn/v2/object/https://pasta.lternet.edu/package/metadata/eml/knb-lter-sbc/4004/6#d_1"/>
        <owl:onProperty rdf:resource="http://ecoinformatics.org/oboe/oboe.1.1/oboe-core.owl#measuresEntity"/>
      </owl:Restriction>
    </rdfs:subClassOf>
    <rdfs:label>Precipitation SBC GB201, all years Date and Time, local</rdfs:label>
    <rdfs:subClassOf>
      <owl:Restriction rdf:nodeID="Nf4ac418a90a94006bb57506d610eb355">
        <owl:onProperty rdf:resource="http://ecoinformatics.org/oboe/oboe.1.1/oboe-core.owl#measuresCharacteristic"/>
        <owl:someValuesFrom rdf:resource="https://cn.dataone.org/cn/v2/object/https://pasta.lternet.edu/package/metadata/eml/knb-lter-sbc/4004/6#d_1_c_1"/>
      </owl:Restriction>
    </rdfs:subClassOf>
    <rdfs:subClassOf rdf:resource="http://ecoinformatics.org/oboe/oboe.1.1/oboe-core.owl#MeasurementType"/>
  </owl:Class>
  <owl:Class rdf:about="https://cn.dataone.org/cn/v2/object/https://pasta.lternet.edu/package/metadata/eml/knb-lter-sbc/4004/6#d_1_c_2">
    <rdfs:comment>local time of observation, no correction for daylight saving time</rdfs:comment>
    <rdfs:subClassOf rdf:resource="http://ecoinformatics.org/oboe/oboe.1.1/oboe-core.owl#Characteristic"/>
    <rdfs:label>Date and Time, local</rdfs:label>
  </owl:Class>
  <owl:Class rdf:about="https://cn.dataone.org/cn/v2/object/https://pasta.lternet.edu/package/metadata/eml/knb-lter-sbc/4004/6#d_1_c_1">
    <rdfs:label>Date and Time, local</rdfs:label>
    <rdfs:subClassOf rdf:resource="http://ecoinformatics.org/oboe/oboe.1.1/oboe-core.owl#Characteristic"/>
    <rdfs:comment>local time of observation, no correction for daylight saving time</rdfs:comment>
  </owl:Class>
  <owl:Class rdf:about="https://cn.dataone.org/cn/v2/object/https://pasta.lternet.edu/package/metadata/eml/knb-lter-sbc/4004/6#d_1">
    <rdfs:subClassOf rdf:resource="http://ecoinformatics.org/oboe/oboe.1.1/oboe-core.owl#Entity"/>
    <rdfs:comment>Precipitation data from Gobernador at Veddar's Ranch (station = GB201) from 2002-10-01 to 2006-09-30.</rdfs:comment>
    <rdfs:label>Precipitation SBC GB201, all years</rdfs:label>
  </owl:Class>
  <owl:Class rdf:about="https://cn.dataone.org/cn/v2/object/https://pasta.lternet.edu/package/metadata/eml/knb-lter-sbc/4004/6#d_1_c_3">
    <rdfs:subClassOf rdf:resource="http://ecoinformatics.org/oboe/oboe.1.1/oboe-core.owl#Characteristic"/>
    <rdfs:label>Date and Time, local</rdfs:label>
    <rdfs:comment>local time of observation, no correction for daylight saving time</rdfs:comment>
  </owl:Class>
</rdf:RDF>
