<?xml version="1.0" encoding="utf-8"?>
<rdf:RDF
  xmlns:owl="http://www.w3.org/2002/07/owl#"
  xmlns:rdf="http://www.w3.org/1999/02/22-rdf-syntax-ns#"
  xmlns:rdfs="http://www.w3.org/2000/01/rdf-schema#"
>
  <owl:Ontology rdf:about="https://cn.dataone.org/cn/v2/object/https://pasta.lternet.edu/package/metadata/eml/knb-lter-arc/10137/3">
    <rdfs:comment>File contains temperature and discharge data for Lake NE 14 Outlet during the 2011 summer field season.</rdfs:comment>
    <rdfs:label>Temperature and discharge data for lake NE 14 Outlet near Toolik Lake, Alaska, during the 2011 summer field season.</rdfs:label>
  </owl:Ontology>
  <owl:Class rdf:about="https://cn.dataone.org/cn/v2/object/https://pasta.lternet.edu/package/metadata/eml/knb-lter-arc/10137/3#d_1_a_1">
    <rdfs:subClassOf>
      <owl:Restriction rdf:nodeID="N42bd6620556e42348bbe6d8e993dd461">
        <owl:onProperty rdf:resource="http://ecoinformatics.org/oboe/oboe.1.1/oboe-core.owl#measuresCharacteristic"/>
        <owl:someValuesFrom rdf:resource="https://cn.dataone.org/cn/v2/object/https://pasta.lternet.edu/package/metadata/eml/knb-lter-arc/10137/3#d_1_c_1"/>
      </owl:Restriction>
    </rdfs:subClassOf>
    <rdfs:subClassOf rdf:resource="http://ecoinformatics.org/oboe/oboe.1.1/oboe-core.owl#MeasurementType"/>
    <rdfs:label>2011_Kling_Thermokarst_NE14_Discharge.csv DateTime</rdfs:label>
    <rdfs:subClassOf>
      <owl:Restriction rdf:nodeID="Ncf50bee7818a4e92936fed5913955c28">
        <owl:onProperty rdf:resource="http://ecoinformatics.org/oboe/oboe.1.1/oboe-core.owl#measuresEntity"/>
        <owl:someValuesFrom rdf:resource="https://cn.dataone.org/cn/v2/object/https://pasta.lternet.edu/package/metadata/eml/knb-lter-arc/10137/3#d_1"/>
      </owl:Restriction>
    </rdfs:subClassOf>
  </owl:Class>
  <owl:Class rdf:about="https://cn.dataone.org/cn/v2/object/https://pasta.lternet.edu/package/metadata/eml/knb-lter-arc/10137/3#d_1_a_3">
    <rdfs:subClassOf>
      <owl:Restriction rdf:nodeID="N6deff4b34c2e4564913f7dfef8c5996b">
        <owl:onProperty rdf:resource="http://ecoinformatics.org/oboe/oboe.1.1/oboe-core.owl#measuresEntity"/>
        <owl:someValuesFrom rdf:resource="https://cn.dataone.org/cn/v2/object/https://pasta.lternet.edu/package/metadata/eml/knb-lter-arc/10137/3#d_1"/>
      </owl:Restriction>
    </rdfs:subClassOf>
    <rdfs:subClassOf>
      <owl:Restriction rdf:nodeID="Nb1786c370df248c698746f1e1410faf2">
        <owl:onProperty rdf:resource="http://ecoinformatics.org/oboe/oboe.1.1/oboe-core.owl#measuresCharacteristic"/>
        <owl:someValuesFrom rdf:resource="https://cn.dataone.org/cn/v2/object/https://pasta.lternet.edu/package/metadata/eml/knb-lter-arc/10137/3#d_1_c_3"/>
      </owl:Restriction>
    </rdfs:subClassOf>
    <rdfs:label>2011_Kling_Thermokarst_NE14_Discharge.csv DateTime</rdfs:label>
    <rdfs:subClassOf rdf:resource="http://ecoinformatics.org/oboe/oboe.1.1/oboe-core.owl#MeasurementType"/>
  </owl:Class>
  <owl:Class rdf:about="https://cn.dataone.org/cn/v2/object/https://pasta.lternet.edu/package/metadata/eml/knb-lter-arc/10137/3#d_1_a_2">
    <rdfs:subClassOf>
      <owl:Restriction rdf:nodeID="N7aa3bd0a49024f07971757e26fecc845">
        <owl:onProperty rdf:resource="http://ecoinformatics.org/oboe/oboe.1.1/oboe-core.owl#measuresCharacteristic"/>
        <owl:someValuesFrom rdf:resource="https://cn.dataone.org/cn/v2/object/https://pasta.lternet.edu/package/metadata/eml/knb-lter-arc/10137/3#d_1_c_2"/>
      </owl:Restriction>
    </rdfs:subClassOf>
    <rdfs:subClassOf rdf:resource="http://ecoinformatics.org/oboe/oboe.1.1/oboe-core.owl#MeasurementType"/>
    <rdfs:subClassOf>
      <owl:Restriction rdf:nodeID="N50e8d8c171c146febfc62e38b7ae0dae">
        <owl:someValuesFrom rdf:resource="https://cn.dataone.org/cn/v2/object/https://pasta.lternet.edu/package/metadata/eml/knb-lter-arc/10137/3#d_1"/>
        <owl:onProperty rdf:resource="http://ecoinformatics.org/oboe/oboe.1.1/oboe-core.owl#measuresEntity"/>
      </owl:Restriction>
    </rdfs:subClassOf>
    <rdfs:label>2011_Kling_Thermokarst_NE14_Discharge.csv DateTime</rdfs:label>
  </owl:Class>
  <owl:Class rdf:about="https://cn.dataone.org/cn/v2/object/https://pasta.lternet.edu/package/metadata/eml/knb-lter-arc/10137/3#d_1_c_2">
    <rdfs:subClassOf rdf:resource="http://ecoinformatics.org/oboe/oboe.1.1/oboe-core.owl#Characteristic"/>
    <rdfs:comment>Sampling Time in Alaska Daylight Savings Time using 24 hour convention. Daylight Savings time is 1 hour ahead of Alaska Standard Time: e.g., if time is 13:00 DST then it is 12:00 AST.</rdfs:comment>
    <rdfs:label>DateTime</rdfs:label>
  </owl:Class>
  <owl:Class rdf:about="https://cn.dataone.org/cn/v2/object/https://pasta.lternet.edu/package/metadata/eml/knb-lter-arc/10137/3#d_1">
    <rdfs:comment>Temperature and discharge data for lake NE 14 Outlet near Toolik Lake, Alaska, during the 2011 summer field season.</rdfs:comment>
    <rdfs:label>2011_Kling_Thermokarst_NE14_Discharge.csv</rdfs:label>
    <rdfs:subClassOf rdf:resource="http://ecoinformatics.org/oboe/oboe.1.1/oboe-core.owl#Entity"/>
  </owl:Class>
  <owl:Class rdf:about="https://cn.dataone.org/cn/v2/object/https://pasta.lternet.edu/package/metadata/eml/knb-lter-arc/10137/3#d_1_c_1">
    <rdfs:label>DateTime</rdfs:label>
    <rdfs:subClassOf rdf:resource="http://ecoinformatics.org/oboe/oboe.1.1/oboe-core.owl#Characteristic"/>
    <rdfs:comment>Sampling Time in Alaska Daylight Savings Time using 24 hour convention. Daylight Savings time is 1 hour ahead of Alaska Standard Time: e.g., if time is 13:00 DST then it is 12:00 AST.</rdfs:comment>
  </owl:Class>
  <owl:Class rdf:about="https://cn.dataone.org/cn/v2/object/https://pasta.lternet.edu/package/metadata/eml/knb-lter-arc/10137/3#d_1_c_3">
    <rdfs:comment>Sampling Time in Alaska Daylight Savings Time using 24 hour convention. Daylight Savings time is 1 hour ahead of Alaska Standard Time: e.g., if time is 13:00 DST then it is 12:00 AST.</rdfs:comment>
    <rdfs:label>DateTime</rdfs:label>
    <rdfs:subClassOf rdf:resource="http://ecoinformatics.org/oboe/oboe.1.1/oboe-core.owl#Characteristic"/>
  </owl:Class>
</rdf:RDF>
